Revert "Feat: Rust operators and immutable collections (#5081)" (#5377)
This reverts commit 3e38580b55ec29c09abf43ee214a1081741f6e23 to fix
failing nightly:
https://github.com/dafny-lang/dafny/actions/runs/8868313153

---------

Co-authored-by: Fabio Madge <fmadge@amazon.com>

Source/DafnyCore/Backends/JavaScript/JavaScriptCodeGenerator.cs
@@ -2570,10 +2570,9 @@ namespace Microsoft.Dafny.Compilers {
       return termLeftWriter;
     }
 
-    protected override void GetCollectionBuilder_Build(CollectionType ct, IToken tok, string collName,
-      ConcreteSyntaxTree wr, ConcreteSyntaxTree wStmt) {
+    protected override string GetCollectionBuilder_Build(CollectionType ct, IToken tok, string collName, ConcreteSyntaxTree wr) {
       // collections are built in place
-      wr.Write(collName);
+      return collName;
     }
 
     protected override void EmitSingleValueGenerator(Expression e, bool inLetExprBody, string type, ConcreteSyntaxTree wr, ConcreteSyntaxTree wStmts) {
