Source/DafnyCore/Options/DafnyCommands.cs
@@ -91,7 +91,6 @@ public static class DafnyCommands {
     CommonOptionBag.QuantifierSyntax,
     CommonOptionBag.UnicodeCharacters,
     CommonOptionBag.UseBaseFileName,
-    CommonOptionBag.EmitUncompilableCode,
     CommonOptionBag.GeneralTraits,
     CommonOptionBag.GeneralNewtypes,
     CommonOptionBag.TypeSystemRefresh,
