Source/DafnyCore/Backends/Rust/Dafny-compiler-rust.dfy
@@ -1,19 +1,15 @@
 include "../Dafny/AST.dfy"
-  // Dafny to Rust compilation tenets:
-  // - The Compiled Dafny AST should be minimal
-  // - The generated code should look idiomatic and close to the original Dafny file if possible
 
 // Rust AST
-module RAST
-  // All ToString methods should produce well-formed Rust code
-{
+module RAST {
   import opened Std.Wrappers
-  import opened DAST.Format
-  import Strings = Std.Strings
+  import opened Std.Strings
 
   const IND := "  "
+  // Indentation level
+  /* trait ModDecl {} */
 
-  datatype Mod =
+  datatype Mod /*extends ModDecl*/ =
       // Rust modules
     | Mod(name: string, body: seq<ModDecl>)
     | ExternMod(name: string)
@@ -39,15 +35,6 @@ module RAST
   {
     if |s| == 0 then "" else
     f(s[0]) + (if |s| > 1 then separator + SeqToString(s[1..], f, separator) else "")
-  }
-  function SeqToHeight<T>(s: seq<T>, f: T --> nat): (r: nat)
-    requires forall t <- s :: f.requires(t)
-    ensures forall t <- s :: f(t) <= r
-  {
-    if |s| == 0 then 0 else
-    var i := f(s[0]);
-    var j := SeqToHeight(s[1..], f);
-    if i < j then j else i
   }
   datatype ModDecl =
     | RawDecl(body: string)
@@ -89,17 +76,9 @@ module RAST
     }
   }
 
-  datatype NamelessFormal =
-    NamelessFormal(visibility: Visibility, tpe: Type)
-  {
-    function ToString(ind: string): string {
-      (if visibility == PUB then "pub " else "") + tpe.ToString(ind)
-    }
-  }
-
   datatype Formals =
     | NamedFormals(fields: seq<Formal>)
-    | NamelessFormals(types: seq<NamelessFormal>)
+    | NamelessFormals(types: seq<Type>)
   {
     function ToString(ind: string, newLine: bool): string {
       if NamedFormals? then
@@ -118,7 +97,7 @@ module RAST
         assert NamelessFormals?;
         var separator := if newLine then ",\n" + ind + IND else ", ";
         "("+
-        SeqToString(types, (t: NamelessFormal) => t.ToString(ind + IND), separator)
+        SeqToString(types, (t: Type) => t.ToString(ind + IND), separator)
         +")"
     }
   }
@@ -149,140 +128,28 @@ module RAST
     }
   }
 
-  type TypeParamConstraint = Type
-
   datatype TypeParam =
-    | RawTypeParam(content: string, constraints: seq<TypeParamConstraint>)
+    | RawTypeParam(content: string)
   {
     static function ToStringMultiple(typeParams: seq<TypeParam>, ind: string): string {
       if |typeParams| == 0 then "" else
-      "<" + SeqToString(typeParams, (t: TypeParam) => t.ToString(ind + IND), ", ") + ">"
-    }
-    static function {:tailrecursion true} AddConstraintsMultiple(
-      typeParams: seq<TypeParam>, constraints: seq<TypeParamConstraint>
-    ): seq<TypeParam> {
-      if |typeParams| == 0 then []
-      else
-        [typeParams[0].AddConstraints(constraints)] + AddConstraintsMultiple(typeParams[1..], constraints)
-    }
-    function AddConstraints(constraints: seq<TypeParamConstraint>): TypeParam {
-      this.(constraints := this.constraints + constraints)
+      "<" + SeqToString(typeParams, (t: TypeParam) => t.ToString(ind + IND), ",") + ">"
     }
     function ToString(ind: string): string {
-      content + (
-        if |constraints| == 0 then
-          ""
-        else
-          ": " + SeqToString(constraints, (t: TypeParamConstraint) requires t < this =>
-                               t.ToString(ind + IND), " + "))
+      content
     }
   }
-  const Self := Borrowed(SelfOwned)
-  const SelfMut := BorrowedMut(SelfOwned)
-  function Rc(underlying: Type): Type {
-    TypeApp(std_type.MSel("rc").MSel("Rc"), [underlying])
-  }
-  function RefCell(underlying: Type): Type {
-    TypeApp(std_type.MSel("cell").MSel("RefCell"), [underlying])
-  }
-  function Vec(underlying: Type): Type {
-    TypeApp(std_type.MSel("vec").MSel("Vec"), [underlying])
-  }
-  function NewVec(elements: seq<Expr>): Expr {
-    Call(Identifier("vec!"), [], elements)
-  }
-  function Clone(underlying: Expr): Expr {
-    Call(Select(underlying, "clone"), [], [])
-  }
-  function Borrow(underlying: Expr): Expr {
-    UnaryOp("&", underlying, UnaryOpFormat.NoFormat)
-  }
-  function BorrowMut(underlying: Expr): Expr {
-    UnaryOp("&mut", underlying, UnaryOpFormat.NoFormat)
-  }
-
-  const CloneTrait := RawType("Clone")
-  const DafnyPrintTrait := RawType("::dafny_runtime::DafnyPrint")
-  const DefaultTrait := RawType("::std::default::Default")
-  const StaticTrait := RawType("'static")
-
-  function RawType(content: string): Type {
-    TIdentifier(content)
-  }
-
   datatype Type =
-    | SelfOwned
-    | U8 | U16 | U32 | U64 | U128 | I8 | I16 | I32 | I64 | I128
-    | TIdentifier(name: string)
-    | TMemberSelect(base: Type, name: string)
-    | TypeApp(baseName: Type, arguments: seq<Type>)
-    | Borrowed(underlying: Type)
-    | BorrowedMut(underlying: Type)
-    | ImplType(underlying: Type)
-    | DynType(underlying: Type)
-    | TupleType(arguments: seq<Type>)
-    | FnType(arguments: seq<Type>, returnType: Type)
-    | IntersectionType(left: Type, right: Type)
+    | Self | SelfOwned | SelfMut
+    | RawType(content: string)
   {
     function ToString(ind: string): string {
-      match this {
-        case TIdentifier(underlying) => underlying
-        case TMemberSelect(underlying, name) => underlying.ToString(ind) + "::" + name
-        case Borrowed(underlying) => "&" + underlying.ToString(ind)
-        case BorrowedMut(underlying) => "&mut " + underlying.ToString(ind)
-        case ImplType(underlying) => "impl " + underlying.ToString(ind)
-        case DynType(underlying) => "dyn " + underlying.ToString(ind)
-        case FnType(arguments, returnType) =>
-          "::std::ops::Fn("+
-          SeqToString(arguments, (arg: Type) requires arg < this =>
-                        arg.ToString(ind + IND), ", ")
-          +") -> " + returnType.ToString(ind + IND)
-        case IntersectionType(left, right) =>
-          left.ToString(ind) + " + " + right.ToString(ind)
-        case TupleType(args) =>
-          (if args == [] then
-             "()"
-           else
-             "(" +
-             SeqToString(args, (arg: Type) requires arg < this => arg.ToString(ind + IND), ", ")
-             + ")")
-        case TypeApp(base, args) =>
-          base.ToString(ind) +
-          (if args == [] then
-             ""
-           else
-             "<" +
-             SeqToString(args, (arg: Type) requires arg < this => arg.ToString(ind + IND), ", ")
-             + ">")
-
-        case SelfOwned() => "Self"
-        case U8() => "u8"
-        case U16() => "u16"
-        case U32() => "u32"
-        case U64() => "u64"
-        case U128() => "u128"
-        case I8() => "i8"
-        case I16() => "i16"
-        case I32() => "i32"
-        case I64() => "i64"
-        case I128() => "i128"
-      }
-    }
-
-    function MSel(name: string): Type {
-      TMemberSelect(this, name)
-    }
-
-    function Apply1(arg: Type): Type {
-      TypeApp(this, [arg])
+      if Self? then "&Self" else
+      if SelfOwned? then "Self" else
+      if SelfMut? then "&mut Self" else
+      content
     }
   }
-
-  const global_type := TIdentifier("")
-  const std_type := global_type.MSel("std")
-  const cell_type := std_type.MSel("cell")
-  const refcell_type := cell_type.MSel("RefCell")
-  const dafny_runtime_type := global_type.MSel("dafny_runtime")
 
   datatype Trait =
     | Trait(typeParams: seq<TypeParam>, tpe: Type, where: string, body: seq<ImplMember>)
@@ -311,7 +178,7 @@ module RAST
   }
   datatype ImplMember =
     | RawImplMember(content: string)
-    | FnDecl(pub: Visibility, fun: Fn)
+    | FnDecl(pub: VISIBILITY, fun: Fn)
   {
     function ToString(ind: string): string {
       if FnDecl? then
@@ -319,15 +186,17 @@ module RAST
       else assert RawImplMember?; content
     }
   }
-  datatype Visibility = PUB | PRIV
+  newtype VISIBILITY = x: int | 0 <= x < 2
+  const PUB := 1 as VISIBILITY
+  const PRIV := 0 as VISIBILITY
 
   datatype Formal =
     Formal(name: string, tpe: Type)
   {
     function ToString(ind: string): string {
       if name == "self" && tpe.SelfOwned? then name
-      else if name == "&self" && tpe == Borrowed(SelfOwned) then name
-      else if name == "&mut self" && tpe == Borrowed(SelfMut) then name
+      else if name == "&self" && tpe.Self? then name
+      else if name == "&mut self" && tpe.SelfMut? then name
       else
         name + ": " + tpe.ToString(ind)
     }
@@ -347,12 +216,7 @@ module RAST
   datatype MatchCase =
     MatchCase(pattern: Pattern, rhs: Expr)
   {
-    ghost function Height(): nat {
-      1 + rhs.Height()
-    }
-    function ToString(ind: string): string
-      decreases Height()
-    {
+    function ToString(ind: string): string {
       var newIndent := if rhs.Block? then ind else ind + IND;
       var rhsString := rhs.ToString(newIndent);
 
@@ -365,13 +229,7 @@ module RAST
   datatype AssignIdentifier =
     AssignIdentifier(identifier: string, rhs: Expr)
   {
-    ghost function Height(): nat {
-      1 + rhs.Height()
-    }
-
-    function ToString(ind: string): string
-      decreases Height()
-    {
+    function ToString(ind: string): string {
       identifier + ": " + rhs.ToString(ind + IND)
     }
   }
@@ -389,468 +247,35 @@ module RAST
       [raw[0]] + AddIndent(raw[1..], ind)
   }
 
-  function max(i: nat, j: nat): nat {
-    if i < j then j else i
-  }
-
-  datatype DeclareType = MUT | CONST
-
-  datatype Associativity = LeftToRight | RightToLeft | RequiresParentheses
-  datatype PrintingInfo =
-    | UnknownPrecedence()
-    | Precedence(precedence: nat)
-    | SuffixPrecedence(precedence: nat)
-    | PrecedenceAssociativity(precedence: nat, associativity: Associativity)
-  {
-    predicate NeedParenthesesFor(underlying: PrintingInfo) {
-      if UnknownPrecedence? then true
-      else if underlying.UnknownPrecedence? then true
-      else if precedence <= underlying.precedence then true
-      else false
-    }
-    predicate NeedParenthesesForLeft(underlying: PrintingInfo) {
-      if UnknownPrecedence? then true
-      else if underlying.UnknownPrecedence? then true
-      else if precedence <= underlying.precedence then
-        precedence < underlying.precedence || !PrecedenceAssociativity? || !associativity.LeftToRight?
-      else false
-    }
-    predicate NeedParenthesesForRight(underlying: PrintingInfo) {
-      if UnknownPrecedence? then true
-      else if underlying.UnknownPrecedence? then true
-      else if precedence <= underlying.precedence then
-        precedence < underlying.precedence || !PrecedenceAssociativity? || !associativity.RightToLeft?
-      else false
-    }
-    lemma Tests()
-      ensures PrecedenceAssociativity(20, LeftToRight)
-              .NeedParenthesesForLeft(PrecedenceAssociativity(20, LeftToRight)) == false
-      ensures PrecedenceAssociativity(20, LeftToRight)
-              .NeedParenthesesForRight(PrecedenceAssociativity(20, LeftToRight)) == true
-      ensures PrecedenceAssociativity(20, RightToLeft)
-              .NeedParenthesesForRight(PrecedenceAssociativity(20, RightToLeft)) == false
-      ensures PrecedenceAssociativity(20, RightToLeft)
-              .NeedParenthesesForLeft(PrecedenceAssociativity(20, RightToLeft)) == true
-      ensures PrecedenceAssociativity(20, LeftToRight)
-              .NeedParenthesesForLeft(PrecedenceAssociativity(30, LeftToRight)) == true
-      ensures PrecedenceAssociativity(20, RightToLeft)
-              .NeedParenthesesForRight(PrecedenceAssociativity(30, RightToLeft)) == true
-    {
-    }
-  }
-
-
   datatype Expr =
       RawExpr(content: string)
-    | Identifier(name: string) // Can be empty for global in MemberSelect
     | Match(matchee: Expr, cases: seq<MatchCase>)
     | StmtExpr(stmt: Expr, rhs: Expr)
     | Block(underlying: Expr)
     | StructBuild(name: string, assignments: seq<AssignIdentifier>)
-    | Tuple(arguments: seq<Expr>)
-    | UnaryOp(op1: string, underlying: Expr, format: Format.UnaryOpFormat)
-    | BinaryOp(op2: string, left: Expr, right: Expr, format2: Format.BinaryOpFormat)
-    | TypeAscription(left: Expr, tpe: Type)
-    | LiteralInt(value: string)
-    | LiteralString(value: string, binary: bool)
-    | ConversionNum(tpe: Type, underlying: Expr)
-    | DeclareVar(declareType: DeclareType, name: string, optType: Option<Type>, optRhs: Option<Expr>)
-    | AssignVar(name: string, rhs: Expr)
-    | IfExpr(cond: Expr, thn: Expr, els: Expr)
-    | Loop(optCond: Option<Expr>, underlying: Expr)
-    | For(name: string, range: Expr, body: Expr)
-    | Labelled(lbl: string, underlying: Expr)
-    | Break(optLbl: Option<string>)
-    | Continue(optLbl: Option<string>)
-    | Return(optExpr: Option<Expr>)
-    | Call(obj: Expr, typeParameters: seq<Type>, arguments: seq<Expr>)
-    | Select(obj: Expr, name: string)
-    | MemberSelect(obj: Expr, name: string)
   {
-    predicate NoExtraSemicolonAfter() {
-      DeclareVar? || AssignVar? || Break? || Continue? || Return? ||
-      (RawExpr? && |content| > 0 && content[|content| - 1] == ';')
-    }
-    // Taken from https://doc.rust-lang.org/reference/expressions.html
-    const printingInfo: PrintingInfo :=
-      match this {
-        case RawExpr(_) => UnknownPrecedence()
-        case Identifier(_) => Precedence(1)
-        case LiteralInt(_) => Precedence(1)
-        case LiteralString(_, _) => Precedence(1)
-        // Paths => Precedence(1)
-        // Method call => Precedence(2)
-        // Field expression => PrecedenceAssociativity(3, LeftToRight)
-        // case function call | ArrayIndexing => Precedence(4)
-        case UnaryOp(op, underlying, format) =>
-          match op {
-            case "?" => SuffixPrecedence(5)
-            case "-" | "*" | "!" | "&" | "&mut" => Precedence(6)
-            case _ => UnknownPrecedence()
-          }
-        case Select(underlying, name) => PrecedenceAssociativity(2, LeftToRight)
-        case MemberSelect(underlying, name) => PrecedenceAssociativity(2, LeftToRight)
-        case Call(_, _, _) => PrecedenceAssociativity(2, LeftToRight)
-        case TypeAscription(left, tpe) =>
-          PrecedenceAssociativity(10, LeftToRight)
-        case BinaryOp(op2, left, right, format) =>
-          match op2 {
-            case "*" | "/" | "%" => PrecedenceAssociativity(20, LeftToRight)
-            case "+" | "-" => PrecedenceAssociativity(30, LeftToRight)
-            case "<<" | ">>" => PrecedenceAssociativity(40, LeftToRight)
-            case "&" => PrecedenceAssociativity(50, LeftToRight)
-            case "^" => PrecedenceAssociativity(60, LeftToRight)
-            case "|" => PrecedenceAssociativity(70, LeftToRight)
-            case "==" | "!=" | "<" | ">" | "<=" | ">=" => PrecedenceAssociativity(80, RequiresParentheses)
-            case "&&" => PrecedenceAssociativity(90, LeftToRight)
-            case "||" => PrecedenceAssociativity(100, LeftToRight)
-            case ".." | "..=" => PrecedenceAssociativity(110, RequiresParentheses)
-            case "=" | "+=" | "-=" | "*=" | "/=" | "%=" | "&=" | "|=" | "^=" | "<<=" | ">>=" =>
-              PrecedenceAssociativity(110, RightToLeft)
-            case _ => PrecedenceAssociativity(0, RequiresParentheses)
-          }
-        case _ => UnknownPrecedence()
-      }
-
-    ghost function Height(): nat {
-      match this {
-        case Identifier(_) => 1
-        case LiteralInt(_) => 1
-        case LiteralString(_, _) => 1
-        case ConversionNum(_, underlying) => 1 + underlying.Height()
-        case Match(matchee, cases) =>
-          1 + max(matchee.Height(),
-                  SeqToHeight(cases, (oneCase: MatchCase)
-                              requires oneCase < this
-                              => oneCase.Height()))
-        case StmtExpr(stmt, rhs) =>
-          var default := 1 + max(stmt.Height(), rhs.Height());
-          match this {
-            case StmtExpr(DeclareVar(mod, name, Some(tpe), None), StmtExpr(AssignVar(name2, rhs), last)) =>
-              if name == name2 then
-                1 + default
-              else default
-            case _ => default
-          }
-
-        case Block(underlying) =>
-          1 + underlying.Height()
-        case StructBuild(name, assignments) =>
-          1 + SeqToHeight(assignments, (assignment: AssignIdentifier)
-                          requires assignment < this
-                          => assignment.Height())
-        case Tuple(arguments) =>
-          1 + SeqToHeight(arguments, (argument: Expr)
-                          requires argument < this
-                          => argument.Height())
-        // Special cases
-        case UnaryOp(_, underlying, _) => 1 + underlying.Height()
-        case TypeAscription(left, tpe) => 1 + left.Height()
-        case BinaryOp(op, left, right, format) =>
-          1 + max(left.Height(), right.Height())
-        case IfExpr(cond, thn, els) =>
-          1 + max(cond.Height(), max(thn.Height(), els.Height()))
-        case DeclareVar(declareType, name, tpe, expr) =>
-          1 + (match expr {
-                 case Some(e) => e.Height()
-                 case None => 0
-               })
-        case AssignVar(name, expr) =>
-          1 + expr.Height()
-        case Loop(optCond, underlying) =>
-          1 + if optCond.Some? then max(optCond.value.Height(), underlying.Height()) else underlying.Height()
-        case Labelled(lbl, underlying) =>
-          1 + underlying.Height()
-        case Break(_) => 1
-        case Continue(_) => 1
-        case For(name, range, body) =>
-          1 + max(range.Height(), body.Height())
-        case Return(optExpr) =>
-          if optExpr.Some? then 1 + optExpr.value.Height() else 1
-        case Call(obj, tpes, args) =>
-          1 + max(obj.Height(),
-                  max(SeqToHeight(tpes, (tpe: Type) requires tpe < this => 1),
-                      SeqToHeight(args, (arg: Expr) requires arg < this => arg.Height())))
-        case Select(expression, name) =>
-          1 + expression.Height()
-        case MemberSelect(expression, name) =>
-          1 + expression.Height()
-        case _ =>
-          assert RawExpr?;
-          1
-      }
-    }
-
-    // Wish: Prove that Optimize() preserves semantics, if any
-    // TODO: Ensure that even without Optimize(), tests pass
-    opaque function Optimize(): (r: Expr)
-      ensures this == r || r.Height() < this.Height()
-    {
-      match this {
-        case UnaryOp("&", Call(Select(underlying, "clone"), typeArgs, args), format) =>
-          if typeArgs == [] && args == [] then
-            assert Select(underlying, "clone").Height() == 1 + underlying.Height();
-            assert Call(Select(underlying, "clone"), typeArgs, args).Height() == 2 + underlying.Height();
-            assert UnaryOp("&", underlying, format).Height() == 1 + underlying.Height();
-            UnaryOp("&", underlying, format)
-          else
-            this
-
-        case UnaryOp("!", BinaryOp("==", left, right, format),
-          CombineFormat()) =>
-          assert BinaryOp("==", left, right, format).Height()
-              == BinaryOp("!=", left, right, BinaryOpFormat.NoFormat()).Height();
-          BinaryOp("!=", left, right, BinaryOpFormat.NoFormat())
-
-        case UnaryOp("!", BinaryOp("<", left, right, NoFormat()),
-          CombineFormat()) =>
-          assert BinaryOp(">=", left, right, BinaryOpFormat.NoFormat()).Height()
-              == BinaryOp("<", left, right, BinaryOpFormat.NoFormat()).Height();
-          BinaryOp(">=", left, right, BinaryOpFormat.NoFormat())
-
-        case UnaryOp("!", BinaryOp("<", left, right, ReverseFormat()),
-          CombineFormat()) =>
-          assert BinaryOp("<=", right, left, BinaryOpFormat.NoFormat()).Height()
-              == BinaryOp("<", left, right, BinaryOpFormat.ReverseFormat()).Height();
-          BinaryOp("<=", right, left, BinaryOpFormat.NoFormat())
-
-        case ConversionNum(tpe, expr) =>
-          if || tpe.U8? || tpe.U16? || tpe.U32? || tpe.U64? || tpe.U128?
-             || tpe.I8? || tpe.I16? || tpe.I32? || tpe.I64? || tpe.I128? then
-            match expr {
-              case Call(MemberSelect(
-                MemberSelect(MemberSelect(
-                Identifier(""), "dafny_runtime"), "DafnyInt"), "from"), tpe, args) =>
-                if |tpe| == 0 && |args| == 1 then
-                  match args[0] {
-                    case LiteralInt(number) => LiteralInt("/*optimized*/"+number)
-                    case LiteralString(number, _) => LiteralInt("/*optimized*/"+number)
-                    case _ => this
-                  }
-                else this
-              case _ => this
-            }
-          else
-            this
-        case StmtExpr(DeclareVar(mod, name, Some(tpe), None), StmtExpr(AssignVar(name2, rhs), last)) =>
-          if name == name2 then
-            var rewriting := StmtExpr(DeclareVar(mod, name, Some(tpe), Some(rhs)), last);
-            assert rewriting.Height() < this.Height() by {
-              assert StmtExpr(AssignVar(name2, rhs), last).Height() ==
-                     1 + max(AssignVar(name2, rhs).Height(), last.Height()) ==
-                     1 + max(1 + rhs.Height(), last.Height());
-              assert this.Height() == 2 + max(1, 1 + max(1 + rhs.Height(), last.Height()));
-              assert rewriting.Height() == 1 + max(1 + rhs.Height(), last.Height());
-            }
-            rewriting
-          else
-            this
-        case _ => this
-      }
-    }
-
-    predicate LeftRequiresParentheses(left: Expr) {
-      printingInfo.NeedParenthesesForLeft(left.printingInfo)
-    }
-    function LeftParentheses(left: Expr): (string, string) {
-      if LeftRequiresParentheses(left) then
-        ("(", ")")
-      else
-        ("", "")
-    }
-
-    predicate RightRequiresParentheses(right: Expr) {
-      printingInfo.NeedParenthesesForRight(right.printingInfo)
-    }
-
-
-    function RightParentheses(right: Expr): (string, string) {
-      if RightRequiresParentheses(right) then
-        ("(", ")")
-      else
-        ("", "")
-    }
-
-    function RightMostIdentifier(): Option<string> {
-      match this {
-        case MemberSelect(_, id) => Some(id)
-        case _ => None
-      }
-    }
-
-    function ToString(ind: string): string
-      decreases Height()
-    {
-      match this.Optimize() {
-        case Identifier(name) => name
-        case LiteralInt(number) => number
-        case LiteralString(characters, binary) =>
-          (if binary then "b" else "") +
-          "\"" + characters + "\""
-        case ConversionNum(tpe, expr) =>
-          if || tpe.U8? || tpe.U16? || tpe.U32? || tpe.U64? || tpe.U128?
-             || tpe.I8? || tpe.I16? || tpe.I32? || tpe.I64? || tpe.I128? then
-            "num::ToPrimitive::to_"+tpe.ToString(ind)+"(" + expr.ToString(ind) + ").unwrap()"
-          else
-            "<b>Unsupported: Numeric conversion to " + tpe.ToString(ind) + "</b>"
-        case Match(matchee, cases) =>
-          "match " + matchee.ToString(ind + IND) + " {" +
-          SeqToString(cases,
-                      (c: MatchCase) requires c.Height() < this.Height() =>
-                        "\n" + ind + IND + c.ToString(ind + IND), ",") +
-          "\n" + ind + "}"
-        case StmtExpr(stmt, rhs) => // They are built like StmtExpr(StmtExpr(StmtExpr(..., 1), 2), 3...)
-          if stmt.RawExpr? && stmt.content == "" then rhs.ToString(ind) else
-          stmt.ToString(ind) + (if stmt.NoExtraSemicolonAfter() then "" else ";") +
-          "\n" + ind + rhs.ToString(ind)
-        case Block(underlying) =>
-          "{\n" + ind + IND + underlying.ToString(ind + IND) + "\n" + ind + "}"
-        case IfExpr(cond, thn, els) =>
-          "if " + cond.ToString(ind + IND) + " {\n" + ind + IND + thn.ToString(ind + IND) +
-          "\n" + ind + "} else {\n" + ind + IND + els.ToString(ind + IND) + "\n" + ind + "}"
-        case StructBuild(name, assignments) =>
-          name + " {" +
-          SeqToString(assignments, (assignment: AssignIdentifier)
-                      requires assignment.Height() < this.Height()
-                      =>
-                        "\n" + ind + IND + assignment.ToString(ind + IND), ",") +
-          (if |assignments| > 0 then "\n" + ind else "") + "}"
-        case Tuple(arguments) =>
-          "(" +
-          SeqToString(arguments, (arg: Expr)
-                      requires arg.Height() < this.Height()
-                      =>
-                        "\n" + ind + IND + arg.ToString(ind + IND), ",") +
-          (if |arguments| > 0 then "\n" + ind else "") + ")"
-
-        case UnaryOp(op, underlying, format) =>
-          var (leftP, rightP) :=
-            if printingInfo.NeedParenthesesFor(underlying.printingInfo) then
-              ("(", ")")
-            else
-              ("", "");
-          var leftOp := if op == "&mut" && leftP != "(" then op + " " else if op == "?" then "" else op;
-          var rightOp := if op == "?" then op else "";
-
-          leftOp + leftP  + underlying.ToString(ind) + rightP + rightOp
-        case TypeAscription(left, tpe) =>
-          var (leftLeftP, leftRightP) := LeftParentheses(left);
-          leftLeftP + left.ToString(IND) + leftRightP + " as " + tpe.ToString(IND)
-        case BinaryOp(op2, left, right, format) =>
-          var (leftLeftP, leftRighP) := LeftParentheses(left);
-          var (rightLeftP, rightRightP) := RightParentheses(right);
-          var opRendered := " " + op2 + " ";
-          var indLeft := if leftLeftP == "(" then ind + IND else ind;
-          var indRight := if rightLeftP == "(" then ind + IND else ind;
-          leftLeftP + left.ToString(indLeft) + leftRighP + opRendered + rightLeftP + right.ToString(indRight) + rightRightP
-        case DeclareVar(declareType, name, optType, optExpr) =>
-          "let " + (if declareType == MUT then "mut " else "") +
-          name + (if optType.Some? then ": " + optType.value.ToString(ind + IND) else "") +
-
-          (if optExpr.Some? then
-             var optExprString := optExpr.value.ToString(ind + IND);
-             if optExprString == "" then
-               "= /*issue with empty RHS*/" +
-               if optExpr.value.RawExpr? then "Empty Raw expr" else
-               if optExpr.value.LiteralString? then "Empty string literal" else
-               if optExpr.value.LiteralInt? then "Empty int literal" else
-               "Another case"
-             else " = " + optExprString else "") + ";"
-        case AssignVar(name, expr) =>
-          name + " = " + expr.ToString(ind + IND) + ";"
-        case Labelled(name, underlying) =>
-          "'" + name + ": " + underlying.ToString(ind)
-        case Break(optLbl) =>
-          match optLbl {
-            case Some(lbl) => "break '" + lbl + ";"
-            case None => "break;"
-          }
-        case Continue(optLbl) =>
-          match optLbl {
-            case Some(lbl) => "continue '" + lbl + ";"
-            case None => "continue;"
-          }
-        case Loop(optCond, underlying) =>
-          (match optCond {
-             case None => "loop"
-             case Some(c) => "while " + c.ToString(ind + IND)
-           }) + " {\n" + ind + IND + underlying.ToString(ind + IND) + "\n" + ind + "}"
-        case For(name, range, body) =>
-          "for "+ name +" in " + range.ToString(ind + IND) + " {\n" + ind + IND +
-          body.ToString(ind + IND) + "\n" + ind + "}"
-        case Return(optExpr) =>
-          "return" + (if optExpr.Some? then " " + optExpr.value.ToString(ind + IND) else "") + ";"
-        case Call(expr, tpes, args) =>
-          var (leftP, rightP) := LeftParentheses(expr);
-          var (leftCallP, rightCallP) := match expr.RightMostIdentifier() {
-            case Some("seq!") | Some("map!")  =>
-              ("[","]")
-            case Some("set!") | Some("multiset!") =>
-              ("{","}")
-            case _ =>
-              ("(", ")")
-          };
-          leftP + expr.ToString(ind) + rightP + (
-            if |tpes| == 0 then ""
-            else
-              "::<" + SeqToString(tpes, (tpe: Type) => tpe.ToString(ind + IND), ", ") +">"
-          ) + leftCallP + SeqToString(args, (arg: Expr) requires arg.Height() < this.Height() => arg.ToString(ind + IND), ", ")+ rightCallP
-        case Select(expression, name) =>
-          var (leftP, rightP) := LeftParentheses(expression);
-          leftP + expression.ToString(ind) + rightP + "." + name
-        case MemberSelect(expression, name) =>
-          var (leftP, rightP) := LeftParentheses(expression);
-          leftP + expression.ToString(ind) + rightP + "::" + name
-        case r =>
-          assert r.RawExpr?; AddIndent(r.content, ind)
-      }
+    function ToString(ind: string): string {
+      if Match? then
+        "match " + matchee.ToString(ind + IND) + " {" +
+        SeqToString(cases, (c: MatchCase) requires c < this =>
+                      "\n" + ind + IND + c.ToString(ind + IND), ",") +
+        "\n" + ind + "}"
+      else if StmtExpr? then
+        stmt.ToString(ind) + ";\n" + ind + rhs.ToString(ind)
+      else if Block? then
+        "{\n" + ind + IND + underlying.ToString(ind + IND) + "\n" + ind + "}"
+      else if StructBuild? then
+        name + " {" +
+        SeqToString(assignments, (assignment: AssignIdentifier)
+                    requires assignment < this
+                    =>
+                      "\n" + ind + IND + assignment.ToString(ind + IND), ",") +
+        (if |assignments| > 0 then "\n" + ind else "") + "}"
+      else assert RawExpr?; AddIndent(content, ind)
     }
     function Then(rhs2: Expr): Expr {
-      if this.StmtExpr? then
-        StmtExpr(stmt, rhs.Then(rhs2))
-      else
-        StmtExpr(this, rhs2)
+      StmtExpr(this, rhs2)
     }
-
-    // Helpers
-
-    function Sel(name: string): Expr {
-      Select(this, name)
-    }
-    function MSel(name: string): Expr {
-      MemberSelect(this, name)
-    }
-
-    function Apply(typeParameters: seq<Type>, arguments: seq<Expr>): Expr {
-      Call(this, typeParameters, arguments)
-    }
-
-    function Apply1(argument: Expr): Expr {
-      Call(this, [], [argument])
-    }
-  }
-
-  const global := Identifier("")
-
-  const dafny_runtime := global.MSel("dafny_runtime")
-  const dafny_runtime_Set := dafny_runtime.MSel("Set")
-  const dafny_runtime_Set_from_array := dafny_runtime_Set.MSel("from_array")
-  const dafny_runtime_Sequence := dafny_runtime.MSel("Sequence")
-  const Sequence_from_array_owned := dafny_runtime_Sequence.MSel("from_array_owned")
-  const Sequence_from_array := dafny_runtime_Sequence.MSel("from_array")
-  const dafny_runtime_Multiset := dafny_runtime.MSel("Multiset")
-  const dafny_runtime_Multiset_from_array := dafny_runtime_Multiset.MSel("from_array")
-
-  const std := global.MSel("std")
-
-  const std_rc := std.MSel("rc")
-
-  const std_rc_Rc := std_rc.MSel("Rc")
-
-  const std_rc_Rc_new := std_rc_Rc.MSel("new")
-
-  function RcNew(underlying: Expr): Expr {
-    Call(std_rc_Rc_new, [], [underlying])
   }
 
   datatype Fn =
@@ -875,15 +300,19 @@ module RAST
   }
 }
 
-module {:extern "DCOMP"} DafnyToRustCompiler {
+module {:extern "DCOMP"} DCOMP {
   import opened DAST
   import Strings = Std.Strings
-  import Std
   import opened Std.Wrappers
   import R = RAST
   const IND := R.IND
   type Type = DAST.Type
   type Formal = DAST.Formal
+
+  function runtime(suffix: string): string {
+    "::dafny_runtime" + suffix
+  }
+  const DafnyErasable := runtime("::DafnyErasable")
 
   // List taken from https://doc.rust-lang.org/book/appendix-01-keywords.html
   const reserved_rust := {
@@ -936,9 +365,7 @@ module {:extern "DCOMP"} DafnyToRustCompiler {
       [i[0]] + replaceDots(i[1..])
   }
 
-  predicate is_tuple_builder(i: string)
-    // A tuple builder identifier looks like ___hMake0 to ___hMake99
-  {
+  predicate is_tuple_builder(i: string) {
     && |i| >= 9
     && i[..8] == "___hMake"
     && i[8] in "0123456789"
@@ -956,7 +383,7 @@ module {:extern "DCOMP"} DafnyToRustCompiler {
     && (|i| >= 2 ==> i[1] != 'T') // To avoid conflict with tuple builders _T<digits>
   }
 
-  predicate is_idiomatic_rust_id(i: string) {
+  predicate is_idiomatic_rust(i: string) {
     0 < |i| && !has_special(i) && i !in reserved_rust
   }
 
@@ -967,7 +394,7 @@ module {:extern "DCOMP"} DafnyToRustCompiler {
       better_tuple_builder_name(i)
     else if i in reserved_rust then
       "r#" + i
-    else if is_idiomatic_rust_id(i) then
+    else if is_idiomatic_rust(i) then
       idiomatic_rust(i)
     else if is_dafny_generated_id(i) then
       i // Dafny-generated identifiers like "_module", cannot be written in Dafny itself
@@ -976,17 +403,8 @@ module {:extern "DCOMP"} DafnyToRustCompiler {
       "r#_" + r
   }
 
-  datatype Ownership = OwnershipOwned | OwnershipBorrowed | OwnershipBorrowedMut | OwnershipAutoBorrowed
-
-
   class COMP {
-    const DafnyChar := if UnicodeChars then "DafnyChar" else "DafnyCharUTF16"
-    const UnicodeChars: bool
-
-    constructor(UnicodeChars: bool) {
-      this.UnicodeChars := UnicodeChars;
-    }
-    method GenModule(mod: Module, containingPath: seq<Ident>) returns (s: R.Mod) {
+    static method GenModule(mod: Module, containingPath: seq<Ident>) returns (s: R.Mod) {
       var body := GenModuleBody(mod.body, containingPath + [Ident.Ident(mod.name)]);
 
       s := if mod.isExtern then
@@ -995,7 +413,7 @@ module {:extern "DCOMP"} DafnyToRustCompiler {
         R.Mod(escapeIdent(mod.name), body);
     }
 
-    method GenModuleBody(body: seq<ModuleItem>, containingPath: seq<Ident>) returns (s: seq<R.ModDecl>) {
+    static method GenModuleBody(body: seq<ModuleItem>, containingPath: seq<Ident>) returns (s: seq<R.ModDecl>) {
       s := [];
       var i := 0;
       while i < |body| {
@@ -1019,36 +437,49 @@ module {:extern "DCOMP"} DafnyToRustCompiler {
       }
     }
 
-    method GenTypeParameters(params: seq<Type>)
+    static method GenTypeParameters(params: seq<Type>)
       returns (
         typeParamsSet: set<Type>,
         typeParams: seq<R.TypeParam>,
         constrainedTypeParams: seq<R.TypeParam>,
-        whereConstraints: string)
+        whereConstraints: string,
+        constrainedEraseParams: seq<R.TypeParam>,
+        unerasedParams: string,
+        erasedParams: string)
     {
       typeParamsSet := {};
       typeParams := [];
       constrainedTypeParams := [];
       whereConstraints := "";
+      constrainedEraseParams := [];
+      unerasedParams := "";
+      erasedParams := "";
       var tpI := 0;
 
       if |params| > 0 {
+        whereConstraints := " where ";
+        unerasedParams := "<";
+        erasedParams := "<";
         while tpI < |params| {
           var tp := params[tpI];
           typeParamsSet := typeParamsSet + {tp};
           var genTp := GenType(tp, false, false);
-          typeParams := typeParams + [R.RawTypeParam(genTp.ToString(IND), [])];
+          typeParams := typeParams + [R.RawTypeParam(genTp)];
+          var baseConstraints := ": ::dafny_runtime::DafnyErasable + ::dafny_runtime::DafnyUnerasable<" + genTp + "> + Clone + ::dafny_runtime::DafnyPrint + ::std::default::Default";
+          constrainedTypeParams := constrainedTypeParams + [R.RawTypeParam(genTp + baseConstraints + " + 'static")];
+          whereConstraints := whereConstraints + "<" + genTp + " as ::dafny_runtime::DafnyErasable>::Erased: ::std::cmp::PartialEq" + ", ";
+          constrainedEraseParams := constrainedEraseParams + [R.RawTypeParam(genTp + "__Erased" + ", " + genTp + baseConstraints + " + ::dafny_runtime::DafnyUnerasable<" + genTp + "__Erased> + 'static")];
+          unerasedParams := unerasedParams + genTp + "__Erased" + ", ";
+          erasedParams := erasedParams + genTp + "::Erased" + ", ";
           tpI := tpI + 1;
         }
+        unerasedParams := unerasedParams + ">";
+        erasedParams := erasedParams + ">";
       }
-      var baseConstraints := [R.CloneTrait, R.DafnyPrintTrait, R.StaticTrait];
-      constrainedTypeParams := R.TypeParam.AddConstraintsMultiple(
-        typeParams, baseConstraints
-      );
     }
 
-    method GenClass(c: Class, path: seq<Ident>) returns (s: seq<R.ModDecl>) {
-      var typeParamsSet, sTypeParams, sConstrainedTypeParams, whereConstraints := GenTypeParameters(c.typeParams);
+    static method GenClass(c: Class, path: seq<Ident>) returns (s: seq<R.ModDecl>) {
+      var typeParamsSet, sTypeParams, sConstrainedTypeParams, whereConstraints, constrainedEraseParams, unerasedParams, erasedParams := GenTypeParameters(c.typeParams);
       var constrainedTypeParams := R.TypeParam.ToStringMultiple(sConstrainedTypeParams, R.IND + R.IND);
 
       var fields: seq<R.Formal> := [];
@@ -1057,15 +488,15 @@ module {:extern "DCOMP"} DafnyToRustCompiler {
       while fieldI < |c.fields| {
         var field := c.fields[fieldI];
         var fieldType := GenType(field.formal.typ, false, false);
-        fields := fields + [R.Formal("pub " + escapeIdent(field.formal.name), R.TypeApp(R.refcell_type, [fieldType]))];
+        fields := fields + [R.Formal("pub " + escapeIdent(field.formal.name), R.RawType("::std::cell::RefCell<" + fieldType + ">"))];
 
         match field.defaultValue {
           case Some(e) => {
-            var eStr, _, _ := GenExpr(e, None, [], OwnershipOwned);
+            var eStr, _, _, _ := GenExpr(e, None, [], true);
             fieldInits := fieldInits + [
               R.AssignIdentifier(
                 escapeIdent(field.formal.name),
-                R.RawExpr("::std::cell::RefCell::new(" + eStr.ToString(IND) + ")"))];
+                R.RawExpr("::std::cell::RefCell::new(" + eStr + ")"))];
           }
           case None => {
             fieldInits := fieldInits + [
@@ -1081,7 +512,7 @@ module {:extern "DCOMP"} DafnyToRustCompiler {
       var typeParamI := 0;
       while typeParamI < |c.typeParams| {
         var tpeGen := GenType(c.typeParams[typeParamI], false, false);
-        fields := fields + [R.Formal("_phantom_type_param_" + Strings.OfNat(typeParamI), R.TypeApp(R.std_type.MSel("marker").MSel("PhantomData"), [tpeGen]))];
+        fields := fields + [R.Formal("_phantom_type_param_" + Strings.OfNat(typeParamI), R.RawType("::std::marker::PhantomData<" + tpeGen + ">"))];
         fieldInits := fieldInits + [
           R.AssignIdentifier(
             "_phantom_type_param_" + Strings.OfNat(typeParamI),
@@ -1091,8 +522,7 @@ module {:extern "DCOMP"} DafnyToRustCompiler {
       }
 
       var struct := R.Struct([], escapeIdent(c.name), sTypeParams, R.NamedFormals(fields));
-      var typeParamsAsTypes :=
-        Std.Collections.Seq.Map((typeParam: R.TypeParam) => R.RawType(typeParam.content), sTypeParams);
+      var typeParams := R.TypeParam.ToStringMultiple(sTypeParams, R.IND + R.IND);
 
       s := [R.StructDecl(struct)];
 
@@ -1112,7 +542,7 @@ module {:extern "DCOMP"} DafnyToRustCompiler {
 
       var i := R.Impl(
         sConstrainedTypeParams,
-        R.TypeApp(R.TIdentifier(escapeIdent(c.name)), typeParamsAsTypes),
+        R.RawType(escapeIdent(c.name) + typeParams),
         whereConstraints,
         implBody
       );
@@ -1134,8 +564,8 @@ module {:extern "DCOMP"} DafnyToRustCompiler {
               var x := R.ImplDecl(
                 R.ImplFor(
                   sConstrainedTypeParams,
-                  R.TypeApp(R.TIdentifier(pathStr), typeArgs),
-                  R.Rc(R.TypeApp(R.TIdentifier(genSelfPath), typeParamsAsTypes)),
+                  R.RawType(pathStr + typeArgs),
+                  R.RawType("::std::rc::Rc<" + genSelfPath + typeParams + ">"),
                   whereConstraints,
                   body
                 ));
@@ -1149,8 +579,8 @@ module {:extern "DCOMP"} DafnyToRustCompiler {
 
       var d := R.ImplFor(
         sConstrainedTypeParams,
-        R.DefaultTrait,
-        R.TypeApp(R.TIdentifier(escapeIdent(c.name)), typeParamsAsTypes),
+        R.RawType("::std::default::Default"),
+        R.RawType(escapeIdent(c.name) + typeParams),
         whereConstraints,
         [R.FnDecl(
            R.PRIV,
@@ -1164,8 +594,8 @@ module {:extern "DCOMP"} DafnyToRustCompiler {
       var p :=
         R.ImplFor(
           sConstrainedTypeParams,
-          R.DafnyPrintTrait,
-          R.TypeApp(R.TIdentifier(escapeIdent(c.name)), typeParamsAsTypes),
+          R.RawType("::dafny_runtime::DafnyPrint"),
+          R.RawType(escapeIdent(c.name) + typeParams),
           "",
           [R.FnDecl(
              R.PRIV,
@@ -1182,7 +612,7 @@ module {:extern "DCOMP"} DafnyToRustCompiler {
       var pp := R.ImplFor(
         sTypeParams,
         R.RawType("::std::cmp::PartialEq"),
-        R.TypeApp(R.TIdentifier(escapeIdent(c.name)), typeParamsAsTypes),
+        R.RawType(escapeIdent(c.name) + typeParams),
         "",
         [R.FnDecl(
            R.PRIV,
@@ -1196,65 +626,96 @@ module {:extern "DCOMP"} DafnyToRustCompiler {
       );
       var ptrPartialEqImpl := [R.ImplDecl(pp)];
 
-      s := s + defaultImpl + printImpl + ptrPartialEqImpl;
+      var ii := R.ImplDecl(R.ImplFor(
+                             sConstrainedTypeParams,
+                             R.RawType("::dafny_runtime::DafnyErasable"),
+                             R.RawType(escapeIdent(c.name) + typeParams),
+                             "",
+                             [R.RawImplMember("type Erased = " + escapeIdent(c.name) + erasedParams + ";")]
+                           ));
+      var u := R.ImplDecl(R.ImplFor(
+                            constrainedEraseParams,
+                            R.RawType("::dafny_runtime::DafnyUnerasable<" + escapeIdent(c.name) + unerasedParams + ">"),
+                            R.RawType(escapeIdent(c.name) + typeParams),
+                            "", []
+                          ));
+      var identEraseImpls := [ii, u];
+
+      s := s + defaultImpl + printImpl + ptrPartialEqImpl + identEraseImpls;
     }
 
-    method GenTrait(t: Trait, containingPath: seq<Ident>) returns (s: string) {
+    static method GenTrait(t: Trait, containingPath: seq<Ident>) returns (s: string) {
       var typeParamsSet := {};
-      var typeParams := [];
+      var typeParams := "";
       var tpI := 0;
       if |t.typeParams| > 0 {
+        typeParams := "<";
         while tpI < |t.typeParams| {
           var tp := t.typeParams[tpI];
           typeParamsSet := typeParamsSet + {tp};
           var genTp := GenType(tp, false, false);
-          typeParams := typeParams + [genTp];
+          typeParams := typeParams + genTp + ", ";
           tpI := tpI + 1;
         }
+        typeParams := typeParams + ">";
       }
 
       var fullPath := containingPath + [Ident.Ident(t.name)];
       var implBody, _ := GenClassImplBody(t.body, true, Type.Path(fullPath, [], ResolvedType.Trait(fullPath)), typeParamsSet);
       s :=
         R.TraitDecl(R.Trait(
-                      [], R.TypeApp(R.TIdentifier(escapeIdent(t.name)), typeParams),
+                      [], R.RawType(escapeIdent(t.name) + typeParams),
                       "",
                       implBody
                     )).ToString(IND);
     }
 
-    method GenNewtype(c: Newtype) returns (s: seq<R.ModDecl>) {
-      var typeParamsSet, sTypeParams, sConstrainedTypeParams, whereConstraints := GenTypeParameters(c.typeParams);
-      var typeParamsAsTypes :=
-        Std.Collections.Seq.Map((t: R.TypeParam) => R.RawType(t.content), sTypeParams);
+    static method GenNewtype(c: Newtype) returns (s: seq<R.ModDecl>) {
+      var typeParamsSet, sTypeParams, sConstrainedTypeParams, whereConstraints, _, _, _ := GenTypeParameters(c.typeParams);
+      var typeParams := R.TypeParam.ToStringMultiple(sTypeParams, R.IND + R.IND);
       var constrainedTypeParams := R.TypeParam.ToStringMultiple(sConstrainedTypeParams, R.IND + R.IND);
 
-      var underlyingType;
-      match NewtypeToRustType(c.base, c.range) {
-        case Some(v) =>
-          underlyingType := v;
-        case None =>
-          underlyingType := GenType(c.base, false, false);
-      }
-      s := [
-        R.StructDecl(
-          R.Struct(
-            [
-              R.RawAttribute("#[derive(Clone, PartialEq)]"),
-              R.RawAttribute("#[repr(transparent)]")
-            ],
-            escapeIdent(c.name),
-            sTypeParams,
-            R.NamelessFormals([R.NamelessFormal(R.PUB, underlyingType)])
-          ))];
+      var underlyingType := GenType(c.base, false, false);
+      s := [R.StructDecl(
+              R.Struct(
+                [
+                  R.RawAttribute("#[derive(Clone, PartialEq)]"),
+                  R.RawAttribute("#[repr(transparent)]")
+                ],
+                escapeIdent(c.name),
+                sTypeParams,
+                R.NamelessFormals([R.RawType("pub " + underlyingType)])
+              ))];
+      s := s +
+      [R.ImplDecl(R.ImplFor(
+                    sConstrainedTypeParams,
+                    R.RawType("::dafny_runtime::DafnyErasable"),
+                    R.RawType(escapeIdent(c.name) + typeParams),
+                    "",
+                    [R.RawImplMember("type Erased = " + underlyingType + ";")]
+                  ))];
+      s := s +
+      [R.ImplDecl(
+         R.ImplFor(
+           sConstrainedTypeParams,
+           R.RawType("::dafny_runtime::DafnyUnerasable<" + underlyingType + ">"),
+           R.RawType(escapeIdent(c.name) + typeParams),
+           "", []))];
+      s := s +
+      [R.ImplDecl(
+         R.ImplFor(
+           sConstrainedTypeParams,
+           R.RawType("::dafny_runtime::DafnyUnerasable<" + escapeIdent(c.name) + typeParams + ">"),
+           R.RawType(escapeIdent(c.name) + typeParams),
+           "", []))];
 
       var fnBody := "";
 
       match c.witnessExpr {
         case Some(e) => {
           // TODO(shadaj): generate statements
-          var eStr, _, _ := GenExpr(e, None, [], OwnershipOwned);
-          fnBody := fnBody + escapeIdent(c.name) + "(" + eStr.ToString(IND) + ")\n";
+          var eStr, _, _, _ := GenExpr(e, None, [], true);
+          fnBody := fnBody + escapeIdent(c.name) + "(" + eStr + ")\n";
         }
         case None => {
           fnBody := fnBody + escapeIdent(c.name) + "(::std::default::Default::default())";
@@ -1273,15 +734,15 @@ module {:extern "DCOMP"} DafnyToRustCompiler {
         R.ImplDecl(
           R.ImplFor(
             sConstrainedTypeParams,
-            R.DefaultTrait,
-            R.TypeApp(R.TIdentifier(escapeIdent(c.name)), typeParamsAsTypes),
+            R.RawType("::std::default::Default"),
+            R.RawType(escapeIdent(c.name) + typeParams),
             whereConstraints,
             [body]))];
       s := s + [
         R.ImplDecl(R.ImplFor(
                      sConstrainedTypeParams,
-                     R.DafnyPrintTrait,
-                     R.TypeApp(R.TIdentifier(escapeIdent(c.name)), typeParamsAsTypes),
+                     R.RawType("::dafny_runtime::DafnyPrint"),
+                     R.RawType(escapeIdent(c.name) + typeParams),
                      "",
                      [R.FnDecl(R.PRIV,
                                R.Fn("fmt_print", [],
@@ -1295,9 +756,9 @@ module {:extern "DCOMP"} DafnyToRustCompiler {
           R.ImplFor(
             sConstrainedTypeParams,
             R.RawType("::std::ops::Deref"),
-            R.TypeApp(R.TIdentifier(escapeIdent(c.name)), typeParamsAsTypes),
+            R.RawType(escapeIdent(c.name) + typeParams),
             "",
-            [R.RawImplMember("type Target = " + underlyingType.ToString(IND) + ";"),
+            [R.RawImplMember("type Target = " + underlyingType + ";"),
              R.FnDecl(
                R.PRIV,
                R.Fn("deref", [],
@@ -1306,11 +767,11 @@ module {:extern "DCOMP"} DafnyToRustCompiler {
                     Some(R.RawExpr("&self.0"))))]))];
     }
 
-    method GenDatatype(c: Datatype) returns (s: seq<R.ModDecl>) {
-      var typeParamsSet, sTypeParams, sConstrainedTypeParams, whereConstraints := GenTypeParameters(c.typeParams);
-      var typeParamsAsTypes :=
-        Std.Collections.Seq.Map((t: R.TypeParam) => R.RawType(t.content), sTypeParams);
+    static method GenDatatype(c: Datatype) returns (s: seq<R.ModDecl>) {
+      var typeParamsSet, sTypeParams, sConstrainedTypeParams, whereConstraints, sConstrainedEraseParams, unerasedParams, erasedParams := GenTypeParameters(c.typeParams);
+      var typeParams := R.TypeParam.ToStringMultiple(sTypeParams, IND + IND);
       var constrainedTypeParams := R.TypeParam.ToStringMultiple(sConstrainedTypeParams, IND + IND);
+      var constrainedEraseParams := R.TypeParam.ToStringMultiple(sConstrainedEraseParams, IND);
 
       var ctors: seq<R.EnumCase> := [];
       var i := 0;
@@ -1322,12 +783,9 @@ module {:extern "DCOMP"} DafnyToRustCompiler {
           var formal := ctor.args[j];
           var formalType := GenType(formal.typ, false, false);
           if c.isCo {
-            ctorArgs := ctorArgs + [
-              R.Formal(escapeIdent(formal.name),
-                       R.TypeApp(R.dafny_runtime_type.MSel("LazyFieldWrapper"), [formalType]))];
+            ctorArgs := ctorArgs + [R.Formal(escapeIdent(formal.name), R.RawType("::dafny_runtime::LazyFieldWrapper<" + formalType + ">"))];
           } else {
-            ctorArgs := ctorArgs + [
-              R.Formal(escapeIdent(formal.name), formalType)];
+            ctorArgs := ctorArgs + [R.Formal(escapeIdent(formal.name), R.RawType(formalType))];
           }
           j := j + 1;
         }
@@ -1402,7 +860,7 @@ module {:extern "DCOMP"} DafnyToRustCompiler {
                 R.PUB,
                 R.Fn(
                   escapeIdent(formal.name),
-                  [], [R.Formal.self], Some(R.Borrowed(formalType)),
+                  [], [R.Formal.self], Some(R.RawType("&" + formalType )),
                   "",
                   Some(methodBody)
                 ))];
@@ -1418,12 +876,11 @@ module {:extern "DCOMP"} DafnyToRustCompiler {
         var types: seq<R.Type> := [];
         while typeI < |c.typeParams| {
           var genTp := GenType(c.typeParams[typeI], false, false);
-          types := types + [R.TypeApp(R.TIdentifier("::std::marker::PhantomData::"), [genTp])];
+          types := types + [R.RawType("::std::marker::PhantomData::<" + genTp + ">")];
           typeI := typeI + 1;
         }
         ctors := ctors + [R.EnumCase("_PhantomVariant",
-                                     R.NamelessFormals(Std.Collections.Seq.Map(
-                                                         tpe => R.NamelessFormal(R.PRIV, tpe), types))
+                                     R.NamelessFormals(types)
                           )];
       }
 
@@ -1437,10 +894,26 @@ module {:extern "DCOMP"} DafnyToRustCompiler {
          R.ImplDecl(
            R.Impl(
              sConstrainedTypeParams,
-             R.TypeApp(R.TIdentifier(escapeIdent(c.name)), typeParamsAsTypes),
+             R.RawType(escapeIdent(c.name) + typeParams),
              whereConstraints,
              implBody
            ))];
+
+      var identEraseImpls :=
+        [R.ImplDecl(
+           R.ImplFor(
+             sConstrainedTypeParams,
+             R.RawType("::dafny_runtime::DafnyErasable"),
+             R.RawType(escapeIdent(c.name) + typeParams),
+             "",
+             [R.RawImplMember("type Erased = " + escapeIdent(c.name) + erasedParams + ";")]
+           )),
+         R.ImplDecl(
+           R.ImplFor(
+             sConstrainedEraseParams,
+             R.RawType("::dafny_runtime::DafnyUnerasable<" + escapeIdent(c.name) + unerasedParams + ">"),
+             R.RawType(escapeIdent(c.name) + typeParams),
+             "", []))];
 
       i := 0;
       var printImplBodyCases: seq<R.MatchCase> := [];
@@ -1492,8 +965,8 @@ module {:extern "DCOMP"} DafnyToRustCompiler {
         R.ImplDecl(
           R.ImplFor(
             sConstrainedTypeParams,
-            R.DafnyPrintTrait,
-            R.TypeApp(R.TIdentifier(escapeIdent(c.name)), typeParamsAsTypes),
+            R.RawType("::dafny_runtime::DafnyPrint"),
+            R.RawType(escapeIdent(c.name) + typeParams),
             "",
             [R.FnDecl(
                R.PRIV,
@@ -1517,16 +990,12 @@ module {:extern "DCOMP"} DafnyToRustCompiler {
           ];
           i := i + 1;
         }
-        var defaultConstrainedTypeParams := R.TypeParam.AddConstraintsMultiple(
-          sTypeParams, [R.DefaultTrait]
-        );
-
         defaultImpl := [
           R.ImplDecl(
             R.ImplFor(
-              defaultConstrainedTypeParams,
-              R.DefaultTrait,
-              R.TypeApp(R.TIdentifier(escapeIdent(c.name)), typeParamsAsTypes),
+              sConstrainedTypeParams,
+              R.RawType("::std::default::Default"),
+              R.RawType(escapeIdent(c.name) + typeParams),
               "",
               [R.FnDecl(
                  R.PRIV,
@@ -1540,7 +1009,7 @@ module {:extern "DCOMP"} DafnyToRustCompiler {
             ))];
       }
 
-      s := enumBody + printImpl + defaultImpl;
+      s := enumBody + identEraseImpls + printImpl + defaultImpl;
     }
 
     static method GenPath(p: seq<Ident>) returns (s: string) {
@@ -1562,146 +1031,129 @@ module {:extern "DCOMP"} DafnyToRustCompiler {
       }
     }
 
-    method GenTypeArgs(args: seq<Type>, inBinding: bool, inFn: bool) returns (s: seq<R.Type>) {
-      s := [];
+    static method GenTypeArgs(args: seq<Type>, inBinding: bool, inFn: bool) returns (s: string) {
+      s := "";
       if |args| > 0 {
+        s := s + "<";
         var i := 0;
         while i < |args| {
+          if i > 0 {
+            s := s + ", ";
+          }
+
           var genTp := GenType(args[i], inBinding, inFn);
-          s := s + [genTp];
+          s := s + genTp;
           i := i + 1;
         }
+        s := s + ">";
       }
     }
 
-    method GenType(c: Type, inBinding: bool, inFn: bool) returns (s: R.Type) {
+    static method GenType(c: Type, inBinding: bool, inFn: bool) returns (s: string) {
       match c {
-        case Path(p, args, resolved) => {
-          var t := GenPath(p);
-          s := R.TIdentifier(t);
+        case Path(p, args, resolved) =>
+          s := GenPath(p);
 
           var typeArgs := GenTypeArgs(args, inBinding, inFn);
-          s := R.TypeApp(s, typeArgs);
+          s := s + typeArgs;
 
           match resolved {
-            case Datatype(_) => {
-              s := R.Rc(s);
-            }
-            case Trait(_) => {
+            case Datatype(_) =>
+              s := "::std::rc::Rc<" + s + ">";
+            case Trait(_) =>
               if p == [Ident.Ident("_System"), Ident.Ident("object")] {
-                s := R.RawType("::std::rc::Rc<dyn ::std::any::Any>");
+                s := "::std::rc::Rc<dyn ::std::any::Any>";
               } else {
                 if inBinding {
                   // impl trait in bindings is not stable
-                  s := R.RawType("_");
+                  s := "_";
                 } else {
-                  s := R.ImplType(s);
+                  s := "impl " + s + "";
                 }
               }
-            }
-            case Newtype(t, range, erased) => {
-              if erased {
-                match NewtypeToRustType(t, range) {
-                  case Some(v) =>
-                    s := v;
-                  case None =>
-                }
-              }
-            }
+            case Primitive =>
           }
-        }
-        case Nullable(inner) => {
-          var innerExpr := GenType(inner, inBinding, inFn);
-          s := R.TypeApp(R.TIdentifier("::std::option::Option"), [innerExpr]);
-        }
-        case Tuple(types) => {
-          var args := [];
-          var i := 0;
-          while i < |types| {
+
+        case Nullable(inner) =>
+          var innerStr := GenType(inner, inBinding, inFn);
+          s := "::std::option::Option<" + innerStr + ">";
+
+        case Tuple(types) =>
+          s := "(";
+          for i := 0 to |types| {
+            if i > 0 {
+              s := s + " ";
+            }
+
             var generated := GenType(types[i], inBinding, inFn);
-            args := args + [generated];
-            i := i + 1;
+            s := s + generated + ",";
           }
-          s := R.TupleType(args);
-        }
-        case Array(element, dims) => {
-          var elem := GenType(element, inBinding, inFn);
-          s := elem;
-          var i := 0;
-          while i < dims {
-            s := R.Rc(R.RefCell(R.Vec(s)));
-            i := i + 1;
+          s := s + ")";
+
+        case Array(element, dims) =>
+          var elemStr := GenType(element, inBinding, inFn);
+          s := elemStr;
+          for i := 0 to dims {
+            s := "::std::rc::Rc<::std::cell::RefCell<::std::vec::Vec<" + s + ">>>";
           }
-        }
-        case Seq(element) => {
-          var elem := GenType(element, inBinding, inFn);
-          s := R.TypeApp(R.dafny_runtime_type.MSel("Sequence"), [elem]);
-        }
-        case Set(element) => {
-          var elem := GenType(element, inBinding, inFn);
-          s := R.TypeApp(R.dafny_runtime_type.MSel("Set"), [elem]);
-        }
-        case Multiset(element) => {
-          var elem := GenType(element, inBinding, inFn);
-          s := R.TypeApp(R.dafny_runtime_type.MSel("Multiset"), [elem]);
-        }
-        case Map(key, value) => {
-          var keyType := GenType(key, inBinding, inFn);
-          var valueType := GenType(value, inBinding, inFn);
-          s := R.TypeApp(R.dafny_runtime_type.MSel("Map"), [keyType, valueType]);
-        }
-        case MapBuilder(key, value) => {
-          var keyType := GenType(key, inBinding, inFn);
-          var valueType := GenType(value, inBinding, inFn);
-          s := R.TypeApp(R.dafny_runtime_type.MSel("MapBuilder"), [keyType, valueType]);
-        }
-        case SetBuilder(elem) => {
-          var elemType := GenType(elem, inBinding, inFn);
-          s := R.TypeApp(R.dafny_runtime_type.MSel("SetBuilder"), [elemType]);
-        }
-        case Arrow(args, result) => {
+
+        case Seq(element) =>
+          var elemStr := GenType(element, inBinding, inFn);
+          s := "::std::vec::Vec<" + elemStr + ">";
+
+        case Set(element) =>
+          var elemStr := GenType(element, inBinding, inFn);
+          s := "::std::collections::HashSet<" + elemStr + ">";
+
+        case Multiset(element) =>
+          var elemStr := GenType(element, inBinding, inFn);
+          s := "::std::collections::HashMap<" + elemStr + ", u64>";
+
+        case Map(key, value) =>
+          var keyStr := GenType(key, inBinding, inFn);
+          var valueStr := GenType(value, inBinding, inFn);
+          s := "::std::collections::HashMap<" + keyStr + ", " + valueStr + ">";
+
+        case Arrow(args, result) =>
           // we cannot use impl until Rc<Fn> impls Fn
           // if inFn || inBinding {
-          //  s := "::dafny_runtime::FunctionWrapper<::std::rc::Rc<dyn ::std::ops::Fn(";
+          s := "::dafny_runtime::FunctionWrapper<::std::rc::Rc<dyn ::std::ops::Fn(";
           // } else {
           //   s := "::dafny_runtime::FunctionWrapper<impl ::std::ops::Fn(";
           // }
-          var argTypes := [];
-          var i := 0;
-          while i < |args| {
+
+          for i := 0 to |args| {
+            if i > 0 {
+              s := s + ", ";
+            }
 
             var generated := GenType(args[i], inBinding, true);
-            argTypes := argTypes + [R.Borrowed(generated)];
-            i := i + 1;
+            s := s + "&" + generated;
           }
 
           var resultType := GenType(result, inBinding, inFn || inBinding);
-          s := R.TypeApp(
-            R.dafny_runtime_type.MSel("FunctionWrapper"),
-            [R.FnType(argTypes, R.IntersectionType(resultType, R.StaticTrait))]);
 
           // if inFn || inBinding {
-          //s := s + ") -> " + resultType + " + 'static>>";
-          // } else {
-          //   s := s + ") -> " + resultType + " + Clone + 'static>";
-          // }
-        }
-        case TypeArg(Ident(name)) => s := R.RawType(escapeIdent(name));
-        case Primitive(p) => {
+          s := s + ") -> " + resultType + " + 'static>>";
+        // } else {
+        //   s := s + ") -> " + resultType + " + Clone + 'static>";
+        // }
+
+        case TypeArg(Ident(name)) => s := escapeIdent(name);
+        case Primitive(p) =>
           match p {
-            case Int => s := R.dafny_runtime_type.MSel("DafnyInt");
-            case Real => s := R.dafny_runtime_type.MSel("BigRational");
-            case String => s := R.TypeApp(R.dafny_runtime_type.MSel("Sequence"),
-                                          [R.dafny_runtime_type.MSel(DafnyChar)]);
-            case Bool => s := R.RawType("bool");
-            case Char => s := R.dafny_runtime_type.MSel(DafnyChar);
+            case Int => s := "::dafny_runtime::BigInt";
+            case Real => s := "::dafny_runtime::BigRational";
+            case String => s := "Vec<char>";
+            case Bool => s := "bool";
+            case Char => s := "char";
           }
-        }
-        case Passthrough(v) => s := R.RawType(v);
+
+        case Passthrough(v) => s := v;
       }
     }
 
-    method GenClassImplBody(body: seq<ClassItem>, forTrait: bool, enclosingType: Type, enclosingTypeParams: set<Type>)
+    static method GenClassImplBody(body: seq<ClassItem>, forTrait: bool, enclosingType: Type, enclosingTypeParams: set<Type>)
       returns (s: seq<R.ImplMember>, traitBodies: map<seq<Ident>, seq<R.ImplMember>>)
     {
       s := [];
@@ -1734,18 +1186,18 @@ module {:extern "DCOMP"} DafnyToRustCompiler {
       }
     }
 
-    method GenParams(params: seq<Formal>) returns (s: seq<R.Formal>) {
+    static method GenParams(params: seq<Formal>) returns (s: seq<R.Formal>) {
       s := [];
       var i := 0;
       while i < |params| {
         var param := params[i];
         var paramType := GenType(param.typ, false, false);
-        s := s + [R.Formal(escapeIdent(param.name), R.Borrowed(paramType))];
+        s := s + [R.Formal(escapeIdent(param.name), R.RawType(" &" + paramType))];
         i := i + 1;
       }
     }
 
-    method GenMethod(m: Method, forTrait: bool, enclosingType: Type, enclosingTypeParams: set<Type>) returns (s: R.ImplMember) {
+    static method GenMethod(m: Method, forTrait: bool, enclosingType: Type, enclosingTypeParams: set<Type>) returns (s: R.ImplMember) {
       var params: seq<R.Formal> := GenParams(m.params);
       var paramNames := [];
       var paramI := 0;
@@ -1758,21 +1210,27 @@ module {:extern "DCOMP"} DafnyToRustCompiler {
         if (forTrait) {
           params := [R.Formal.self] + params;
         } else {
-          var tpe := GenType(enclosingType, false, false);
-          params := [R.Formal("self", R.Borrowed(tpe))] + params;
+          var enclosingTypeString := GenType(enclosingType, false, false);
+          params := [R.Formal("self", R.RawType("&" + enclosingTypeString))] + params;
         }
       }
 
-      // TODO: Use mut instead of a tuple for the API of multiple output parameters
-      var retTypeArgs := [];
-      //var retType := if |m.outTypes| != 1 then "(" else "";
+      var retType := if |m.outTypes| != 1 then "(" else "";
 
       var typeI := 0;
       while typeI < |m.outTypes| {
-        var typeExpr := GenType(m.outTypes[typeI], false, false);
-        retTypeArgs := retTypeArgs + [typeExpr];
+        if typeI > 0 {
+          retType := retType + ", ";
+        }
+
+        var typeString := GenType(m.outTypes[typeI], false, false);
+        retType := retType + typeString;
 
         typeI := typeI + 1;
+      }
+
+      if |m.outTypes| != 1 {
+        retType := retType + ")";
       }
 
       var visibility := R.PUB;//if forTrait then R.PUB else R.PRIV;
@@ -1798,15 +1256,15 @@ module {:extern "DCOMP"} DafnyToRustCompiler {
 
         var i := 0;
         while i < |typeParamsFiltered| {
+          if i > 0 {
+            whereClauses := whereClauses + ", ";
+          }
 
-          var typeExpr := GenType(typeParamsFiltered[i], false, false);
+          var typeString := GenType(typeParamsFiltered[i], false, false);
           typeParams := typeParams + [
-            R.RawTypeParam(typeExpr.ToString(IND),
-                           [R.CloneTrait,
-                            R.DafnyPrintTrait,
-                            R.DefaultTrait,
-                            R.StaticTrait])
+            R.RawTypeParam(typeString + ": ::dafny_runtime::DafnyErasable + ::dafny_runtime::DafnyUnerasable<" + typeString + "> + Clone + ::dafny_runtime::DafnyPrint + ::std::default::Default + 'static")
           ];
+          whereClauses := whereClauses + "<" + typeString + " as ::dafny_runtime::DafnyErasable>::Erased: ::std::cmp::PartialEq";
 
           i := i + 1;
         }
@@ -1815,28 +1273,29 @@ module {:extern "DCOMP"} DafnyToRustCompiler {
       var fBody: Option<R.Expr>;
 
       if m.hasBody {
-        var earlyReturn: R.Expr := R.Return(None);
+        var earlyReturn := "return;";
         match m.outVars {
           case Some(outVars) => {
-
-            var tupleArgs := [];
-
+            earlyReturn := "return (";
             var outI := 0;
             while outI < |outVars| {
+              if outI > 0 {
+                earlyReturn := earlyReturn + ", ";
+              }
 
               var outVar := outVars[outI];
-              tupleArgs := tupleArgs + [R.Identifier(escapeIdent(outVar.id))];
+              earlyReturn := earlyReturn + escapeIdent(outVar.id);
 
               outI := outI + 1;
             }
-            earlyReturn := R.Return(Some(R.Tuple(tupleArgs)));
+            earlyReturn := earlyReturn + ");";
           }
           case None => {}
         }
 
         var body, _ := GenStmts(m.body, if m.isStatic then None else Some("self"), paramNames, true, earlyReturn);
 
-        fBody := Some(body);
+        fBody := Some(R.RawExpr(body));
       } else {
         fBody := None;
       }
@@ -1846,23 +1305,21 @@ module {:extern "DCOMP"} DafnyToRustCompiler {
           fnName,
           typeParams,
           params,
-          Some(if |retTypeArgs| == 1 then retTypeArgs[0] else R.TupleType(retTypeArgs)),
+          Some(R.RawType(retType)),
           whereClauses,
           fBody
         )
       );
     }
 
-    method GenStmts(stmts: seq<Statement>, selfIdent: Option<string>, params: seq<string>, isLast: bool, earlyReturn: R.Expr) returns (generated: R.Expr, readIdents: set<string>)
-      decreases stmts, 1
-    {
-      generated := R.RawExpr("");
+    static method GenStmts(stmts: seq<Statement>, selfIdent: Option<string>, params: seq<string>, isLast: bool, earlyReturn: string) returns (generated: string, readIdents: set<string>) {
+      generated := "";
       var declarations := {};
       readIdents := {};
       var i := 0;
       while i < |stmts| {
         var stmt := stmts[i];
-        var stmtExpr, recIdents := GenStmt(stmt, selfIdent, params, isLast && (i == |stmts| - 1), earlyReturn);
+        var stmtString, recIdents := GenStmt(stmt, selfIdent, params, isLast && (i == |stmts| - 1), earlyReturn);
         readIdents := readIdents + (recIdents - declarations);
 
         match stmt {
@@ -1871,15 +1328,17 @@ module {:extern "DCOMP"} DafnyToRustCompiler {
           }
           case _ => {}
         }
-        generated := generated.Then(stmtExpr);
 
+        if i > 0 {
+          generated := generated + "\n";
+        }
+
+        generated := generated + stmtString;
         i := i + 1;
       }
     }
 
-    method GenAssignLhs(lhs: AssignLhs, rhs: string, selfIdent: Option<string>, params: seq<string>) returns (generated: string, needsIIFE: bool, readIdents: set<string>)
-      decreases lhs, 1
-    {
+    static method GenAssignLhs(lhs: AssignLhs, rhs: string, selfIdent: Option<string>, params: seq<string>) returns (generated: string, needsIIFE: bool, readIdents: set<string>) {
       match lhs {
         case Ident(Ident(id)) => {
           if id in params {
@@ -1893,30 +1352,33 @@ module {:extern "DCOMP"} DafnyToRustCompiler {
         }
 
         case Select(on, field) => {
-          var onExpr, onOwned, recIdents := GenExpr(on, selfIdent, params, OwnershipBorrowed);
-          generated := "*(" + onExpr.ToString(IND) + "." + field + ".borrow_mut()) = " + rhs + ";";
+          var onExpr, onOwned, onErased, recIdents := GenExpr(on, selfIdent, params, false);
+          generated := "*(" + onExpr + "." + field + ".borrow_mut()) = " + rhs + ";";
           readIdents := recIdents;
           needsIIFE := true;
         }
 
         case Index(on, indices) => {
-          var onExpr, onOwned, recIdents := GenExpr(on, selfIdent, params, OwnershipBorrowed);
+          var onExpr, onOwned, onErased, recIdents := GenExpr(on, selfIdent, params, false);
           readIdents := recIdents;
 
           generated := "{\n";
 
           var i := 0;
           while i < |indices| {
-            var idx, _, recIdentsIdx := GenExpr(indices[i], selfIdent, params, OwnershipOwned);
+            var idx, _, idxErased, recIdentsIdx := GenExpr(indices[i], selfIdent, params, true);
+            if !idxErased {
+              idx := "::dafny_runtime::DafnyErasable::erase_owned(" + idx + ")";
+            }
 
-            generated := generated + "let __idx" + Strings.OfNat(i) + " = <usize as ::dafny_runtime::NumCast>::from(" + idx.ToString(IND) + ").unwrap();\n";
+            generated := generated + "let __idx" + Strings.OfNat(i) + " = <usize as ::dafny_runtime::NumCast>::from(" + idx + ").unwrap();\n";
 
             readIdents := readIdents + recIdentsIdx;
 
             i := i + 1;
           }
 
-          generated := generated + onExpr.ToString(IND) + ".borrow_mut()";
+          generated := generated + onExpr + ".borrow_mut()";
           i := 0;
           while i < |indices| {
             generated := generated + "[__idx" + Strings.OfNat(i) + "]";
@@ -1929,108 +1391,121 @@ module {:extern "DCOMP"} DafnyToRustCompiler {
       }
     }
 
-    method GenStmt(stmt: Statement, selfIdent: Option<string>, params: seq<string>, isLast: bool, earlyReturn: R.Expr) returns (generated: R.Expr, readIdents: set<string>)
-      decreases stmt, 1
-    {
+    static method GenStmt(stmt: Statement, selfIdent: Option<string>, params: seq<string>, isLast: bool, earlyReturn: string) returns (generated: string, readIdents: set<string>) {
       match stmt {
         case DeclareVar(name, typ, Some(expression)) => {
           var typeString := GenType(typ, true, false);
-          var expr, _, recIdents := GenExpr(expression, selfIdent, params, OwnershipOwned);
+          var expr, _, recErased, recIdents := GenExpr(expression, selfIdent, params, true);
+          if !recErased {
+            expr := "::dafny_runtime::DafnyErasable::erase_owned(" + expr + ")";
+          }
 
-          generated := R.DeclareVar(R.MUT, escapeIdent(name), Some(typeString), Some(expr));
+          expr := "<" + typeString + " as ::dafny_runtime::DafnyUnerasable<_>>::unerase_owned(" + expr + ")";
+
+          generated := "let mut " + escapeIdent(name) + ": " + typeString + " = " + expr + ";";
           readIdents := recIdents;
         }
         case DeclareVar(name, typ, None) => {
           var typeString := GenType(typ, true, false);
-          generated := R.DeclareVar(R.MUT, escapeIdent(name), Some(typeString), None);
+          generated := "let mut " + escapeIdent(name) + ": " + typeString + ";";
           readIdents := {};
         }
         case Assign(lhs, expression) => {
           var lhsGen, needsIIFE, recIdents := GenAssignLhs(lhs, "__rhs", selfIdent, params);
-          var exprGen, _, exprIdents := GenExpr(expression, selfIdent, params, OwnershipOwned);
+          var exprGen, _, exprErased, exprIdents := GenExpr(expression, selfIdent, params, true);
+          if !exprErased {
+            exprGen := "::dafny_runtime::DafnyErasable::erase_owned(" + exprGen + ")";
+          }
+
+          exprGen := "::dafny_runtime::DafnyUnerasable::<_>::unerase_owned(" + exprGen + ")";
 
           if needsIIFE {
-            generated := R.Block(
-              R.StmtExpr(
-                R.DeclareVar(R.CONST, "__rhs", None, Some(exprGen)),
-                R.RawExpr(lhsGen)
-              )
-            );
+            generated := "{\nlet __rhs = " + exprGen + ";\n" + lhsGen + "\n}";
           } else {
-            generated := R.AssignVar(lhsGen, exprGen);
+            generated := lhsGen + " = " + exprGen + ";";
           }
 
           readIdents := recIdents + exprIdents;
         }
         case If(cond, thn, els) => {
-          var cond, _, recIdents := GenExpr(cond, selfIdent, params, OwnershipOwned);
-          var condString := cond.ToString(IND);
+          var condString, _, condErased, recIdents := GenExpr(cond, selfIdent, params, true);
+          if !condErased {
+            condString := "::dafny_runtime::DafnyErasable::erase_owned(" + condString + ")";
+          }
 
           readIdents := recIdents;
-          var thn, thnIdents := GenStmts(thn, selfIdent, params, isLast, earlyReturn);
+          var thnString, thnIdents := GenStmts(thn, selfIdent, params, isLast, earlyReturn);
           readIdents := readIdents + thnIdents;
-          var els, elsIdents := GenStmts(els, selfIdent, params, isLast, earlyReturn);
+          var elsString, elsIdents := GenStmts(els, selfIdent, params, isLast, earlyReturn);
           readIdents := readIdents + elsIdents;
-          generated := R.IfExpr(cond, thn, els);
+          generated := "if " + condString + " {\n" + thnString + "\n} else {\n" + elsString + "\n}";
         }
         case Labeled(lbl, body) => {
-          var body, bodyIdents := GenStmts(body, selfIdent, params, isLast, earlyReturn);
+          var bodyString, bodyIdents := GenStmts(body, selfIdent, params, isLast, earlyReturn);
           readIdents := bodyIdents;
-          generated := R.Labelled("label_" + lbl, R.Loop(None, R.StmtExpr(body, R.Break(None))));
+          generated := "'label_" + lbl + ": loop {\n" + bodyString + "\n" + "break;" + "\n}";
         }
         case While(cond, body) => {
-          var cond, _, recIdents := GenExpr(cond, selfIdent, params, OwnershipOwned);
+          var condString, _, condErased, recIdents := GenExpr(cond, selfIdent, params, true);
+          if !condErased {
+            condString := "::dafny_runtime::DafnyErasable::erase_owned(" + condString + ")";
+          }
 
           readIdents := recIdents;
-          var body, bodyIdents := GenStmts(body, selfIdent, params, false, earlyReturn);
+          var bodyString, bodyIdents := GenStmts(body, selfIdent, params, false, earlyReturn);
           readIdents := readIdents + bodyIdents;
 
-          generated := R.Loop(Some(cond), body);
+          generated := "while " + condString + " {\n" + bodyString + "\n}";
         }
         case Foreach(boundName, boundType, over, body) => {
-          var over, _, recIdents := GenExpr(over, selfIdent, params, OwnershipOwned);
+          var overString, _, overErased, recIdents := GenExpr(over, selfIdent, params, true);
 
           var boundTypeStr := GenType(boundType, false, false);
 
           readIdents := recIdents;
-          var body, bodyIdents := GenStmts(body, selfIdent, params + [boundName], false, earlyReturn);
+          var bodyString, bodyIdents := GenStmts(body, selfIdent, params + [boundName], false, earlyReturn);
           readIdents := readIdents + bodyIdents - {boundName};
 
-          generated := R.For(escapeIdent(boundName), over, body);
+          var unerasedIter := "_iter_erased";
+          if overErased {
+            unerasedIter := "<" + boundTypeStr + " as ::dafny_runtime::DafnyUnerasable<_>>::unerase_owned(" + unerasedIter + ")";
+          }
+
+          generated := "for _iter_erased in " + overString + " {\n";
+          generated := generated + "let " + escapeIdent(boundName) + " = " + unerasedIter + ";\n" + bodyString + "\n}";
         }
         case Break(toLabel) => {
           match toLabel {
             case Some(lbl) => {
-              generated := R.Break(Some("label_" + lbl));
+              generated := "break 'label_" + lbl + ";";
             }
             case None => {
-              generated := R.Break(None);
+              generated := "break;";
             }
           }
           readIdents := {};
         }
         case TailRecursive(body) => {
           // clone the parameters to make them mutable
-          generated := R.RawExpr("");
+          generated := "";
 
           if selfIdent != None {
-            generated := generated.Then(R.DeclareVar(R.MUT, "_this", None, Some(R.RawExpr("self.clone()"))));
+            generated := generated + "let mut _this = self.clone();\n";
           }
 
           var paramI := 0;
           while paramI < |params| {
             var param := params[paramI];
-            generated := generated.Then(R.DeclareVar(R.MUT, escapeIdent(param), None, Some(R.Clone(R.Identifier(escapeIdent(param))))));
+            generated := generated + "let mut " + escapeIdent(param) + " = " + escapeIdent(param) + ".clone();\n";
             paramI := paramI + 1;
           }
 
-          var body, bodyIdents := GenStmts(body, if selfIdent != None then Some("_this") else None, [], false, earlyReturn);
+          var bodyString, bodyIdents := GenStmts(body, if selfIdent != None then Some("_this") else None, [], false, earlyReturn);
           readIdents := bodyIdents;
-          generated := generated.Then(R.Labelled("TAIL_CALL_START",
-                                                 R.Loop(None, body)));
+          generated := generated + "'TAIL_CALL_START: loop {\n" + bodyString + "\n}";
         }
         case JumpTailCallStart() => {
-          generated := R.Continue(Some("TAIL_CALL_START"));
+          generated := "continue 'TAIL_CALL_START;";
           readIdents := {};
         }
         case Call(on, name, typeArgs, args, maybeOutVars) => {
@@ -2039,14 +1514,18 @@ module {:extern "DCOMP"} DafnyToRustCompiler {
           var typeArgString := "";
           if (|typeArgs| >= 1) {
             var typeI := 0;
-            var typeArgsR := [];
+            typeArgString := "::<";
             while typeI < |typeArgs| {
-              var tpe := GenType(typeArgs[typeI], false, false);
-              typeArgsR := typeArgsR + [tpe];
+              if typeI > 0 {
+                typeArgString := typeArgString + ", ";
+              }
+
+              var typeString := GenType(typeArgs[typeI], false, false);
+              typeArgString := typeArgString + typeString;
 
               typeI := typeI + 1;
             }
-            typeArgString := R.TypeApp(R.TIdentifier("::"), typeArgsR).ToString(IND);
+            typeArgString := typeArgString + ">";
           }
 
           var argString := "";
@@ -2056,18 +1535,22 @@ module {:extern "DCOMP"} DafnyToRustCompiler {
               argString := argString + ", ";
             }
 
-            var argExpr, ownership, argIdents := GenExpr(args[i], selfIdent, params, OwnershipBorrowed);
-            var argExprString := argExpr.ToString(IND);
+            var argExpr, isOwned, argErased, argIdents := GenExpr(args[i], selfIdent, params, false);
+            if argErased {
+              argExpr := "::dafny_runtime::DafnyUnerasable::<_>::unerase_owned(" + argExpr + ")";
+            }
+            if isOwned {
+              argExpr := "&" + argExpr;
+            }
 
-            argString := argString + argExprString;
+            argString := argString + argExpr;
             readIdents := readIdents + argIdents;
 
             i := i + 1;
           }
 
-          var onExpr, _, enclosingIdents := GenExpr(on, selfIdent, params, OwnershipAutoBorrowed);
+          var enclosingString, _, _, enclosingIdents := GenExpr(on, selfIdent, params, false);
           readIdents := readIdents + enclosingIdents;
-          var enclosingString := onExpr.ToString(IND);
           match on {
             case Companion(_) => {
               enclosingString := enclosingString + "::";
@@ -2101,24 +1584,19 @@ module {:extern "DCOMP"} DafnyToRustCompiler {
             case None => {}
           }
 
-          var renderedName := match name {
-            case Name(name) => escapeIdent(name)
-            case MapBuilderAdd() | SetBuilderAdd() => "add"
-            case MapBuilderBuild() | SetBuilderBuild() => "build"
-          };
-
-          generated := R.RawExpr(
+          generated :=
             (if receiver != "" then (receiver + " = ") else "") +
-            enclosingString + renderedName + typeArgString + "(" + argString + ");");
+            enclosingString + escapeIdent(name) + typeArgString + "(" + argString + ");";
         }
         case Return(expr) => {
-          var expr, _, recIdents := GenExpr(expr, selfIdent, params, OwnershipOwned);
+          var exprString, _, recErased, recIdents := GenExpr(expr, selfIdent, params, true);
+          exprString := "::dafny_runtime::DafnyUnerasable::<_>::unerase_owned(::dafny_runtime::DafnyErasable::erase_owned(" + exprString + "))";
           readIdents := recIdents;
 
           if isLast {
-            generated := expr;
+            generated := exprString;
           } else {
-            generated := R.Return(Some(expr));
+            generated := "return " + exprString + ";";
           }
         }
         case EarlyReturn() => {
@@ -2126,614 +1604,118 @@ module {:extern "DCOMP"} DafnyToRustCompiler {
           readIdents := {};
         }
         case Halt() => {
-          generated := R.RawExpr("panic!(\"Halt\");");
+          generated := "panic!(\"Halt\");";
           readIdents := {};
         }
         case Print(e) => {
-          var printedExpr, recOwnership, recIdents := GenExpr(e, selfIdent, params, OwnershipBorrowed);
-          var printedExprString := printedExpr.ToString(IND);
-          generated := R.RawExpr("print!(\"{}\", ::dafny_runtime::DafnyPrintWrapper(" + printedExprString + "));");
+          var printedExpr, isOwned, _, recIdents := GenExpr(e, selfIdent, params, false);
+          if isOwned {
+            printedExpr := "&(" + printedExpr + ")";
+          }
+          generated := "print!(\"{}\", ::dafny_runtime::DafnyPrintWrapper(" + printedExpr + "));";
           readIdents := recIdents;
         }
       }
     }
 
-    static const OpTable: map<BinOp, string>
-      :=
-      map[
-        Mod() := "%",
-        And() := "&&",
-        Or() := "||",
-        Div() := "/",
-        Lt() := "<",
-        LtChar() := "<",
-        Plus() := "+",
-        Minus() := "-",
-        Times() := "*",
-        BitwiseAnd() := "&",
-        BitwiseOr() := "|",
-        BitwiseXor() := "^",
-        BitwiseShiftRight() := ">>",
-        BitwiseShiftLeft() := "<<"
-      ]
-
-    static function NewtypeToRustType(base: Type, range: NewtypeRange)
-      : Option<R.Type> {
-      match range {
-        case NoRange() => None
-        case U8() => Some(R.Type.U8)
-        case U16() => Some(R.Type.U16)
-        case U32() => Some(R.Type.U32)
-        case U64() => Some(R.Type.U64)
-        case U128() => Some(R.Type.U128)
-        case I8() => Some(R.Type.I8)
-        case I16() => Some(R.Type.I16)
-        case I32() => Some(R.Type.I32)
-        case I64() => Some(R.Type.I64)
-        case I128() => Some(R.Type.I128)
-        case _ => None
-      }
-    }
-
-    static method FromOwned(r: R.Expr, expectedOwnership: Ownership)
-      returns (out: R.Expr, resultingOwnership: Ownership)
-      ensures resultingOwnership != OwnershipAutoBorrowed
-      ensures expectedOwnership != OwnershipAutoBorrowed
-              ==> resultingOwnership == expectedOwnership
-    {
-      if expectedOwnership == OwnershipOwned || expectedOwnership == OwnershipAutoBorrowed {
-        out := r;
-        resultingOwnership := OwnershipOwned;
-      } else if expectedOwnership == OwnershipBorrowed {
-        out := R.Borrow(r);
-        resultingOwnership := OwnershipBorrowed;
-      } else {
-        assert expectedOwnership == OwnershipBorrowedMut;
-        out := R.BorrowMut(r);
-        resultingOwnership := OwnershipBorrowedMut;
-      }
-    }
-
-    static method FromOwnership(r: R.Expr, ownership: Ownership, expectedOwnership: Ownership)
-      returns (out: R.Expr, resultingOwnership: Ownership)
-      requires ownership != OwnershipAutoBorrowed
-      ensures OwnershipGuarantee(expectedOwnership, resultingOwnership)
-    {
-      if ownership == OwnershipOwned {
-        out, resultingOwnership := FromOwned(r, expectedOwnership);
-        return;
-      } else if ownership == OwnershipBorrowed || ownership == OwnershipBorrowedMut {
-        if expectedOwnership == OwnershipOwned {
-          resultingOwnership := OwnershipOwned;
-          out := R.Clone(r);
-        } else if expectedOwnership == ownership
-                  || expectedOwnership == OwnershipAutoBorrowed {
-          resultingOwnership := ownership;
-          out := r;
-        } else if expectedOwnership == OwnershipBorrowed
-                  && ownership == OwnershipBorrowedMut {
-          resultingOwnership := OwnershipBorrowed;
-          out := r;
-        } else {
-          assert expectedOwnership == OwnershipBorrowedMut;
-          resultingOwnership := OwnershipBorrowedMut;
-          out := R.BorrowMut(r); // Not sure if it will ever happen
-        }
-      } else {
-        assert false;
-      }
-    }
-
-    static predicate OwnershipGuarantee(expectedOwnership: Ownership, resultingOwnership: Ownership) {
-      && (expectedOwnership != OwnershipAutoBorrowed ==>
-            resultingOwnership == expectedOwnership)
-      && resultingOwnership != OwnershipAutoBorrowed // We know what's going on
-    }
-
-    method GenExprLiteral(
-      e: Expression,
-      selfIdent: Option<string>,
-      params: seq<string>,
-      expectedOwnership: Ownership
-    ) returns (r: R.Expr, resultingOwnership: Ownership, readIdents: set<string>)
-      requires e.Literal?
-      ensures OwnershipGuarantee(expectedOwnership, resultingOwnership)
-      decreases e, 0
-    {
+    static method GenExpr(e: Expression, selfIdent: Option<string>, params: seq<string>, mustOwn: bool) returns (s: string, isOwned: bool, isErased: bool, readIdents: set<string>)
+      ensures mustOwn ==> isOwned
+      decreases e {
       match e {
         case Literal(BoolLiteral(false)) => {
-          r, resultingOwnership :=
-            FromOwned(R.RawExpr("false"), expectedOwnership);
+          s := "false";
+          isOwned := true;
+          isErased := false;
           readIdents := {};
-          return;
         }
         case Literal(BoolLiteral(true)) => {
-          r, resultingOwnership :=
-            FromOwned(R.RawExpr("true"), expectedOwnership);
+          s := "true";
+          isOwned := true;
+          isErased := false;
           readIdents := {};
-          return;
         }
         case Literal(IntLiteral(i, t)) => {
           match t {
             case Primitive(Int) => {
-              if |i| <= 4 {
-                r := R.dafny_runtime.MSel("DafnyInt").MSel("from").Apply1(R.LiteralInt(i));
-              } else {
-                r := R.dafny_runtime.MSel("DafnyInt").MSel("from").Apply1(
-                  R.LiteralString(i, binary := true));
-              }
+              s := "::dafny_runtime::BigInt::parse_bytes(b\"" + i + "\", 10).unwrap()";
             }
             case o => {
               var genType := GenType(o, false, false);
-              r := R.TypeAscription(R.RawExpr(i), genType);
+              s := "(" + i + " as " + genType + ")";
             }
           }
-          r, resultingOwnership := FromOwned(r, expectedOwnership);
+
+          isOwned := true;
+          isErased := false;
           readIdents := {};
-          return;
         }
         case Literal(DecLiteral(n, d, t)) => {
           match t {
             case Primitive(Real) => {
-              r := R.RcNew(R.RawExpr("::dafny_runtime::BigRational::new(::dafny_runtime::BigInt::parse_bytes(b\"" + n + "\", 10).unwrap(), ::dafny_runtime::BigInt::parse_bytes(b\"" + d + "\", 10).unwrap())"));
+              s := "::dafny_runtime::BigRational::new(::dafny_runtime::BigInt::parse_bytes(b\"" + n + "\", 10).unwrap(), ::dafny_runtime::BigInt::parse_bytes(b\"" + d + "\", 10).unwrap())";
             }
             case o => {
               var genType := GenType(o, false, false);
-              r := R.TypeAscription(R.RawExpr("(" + n + ".0 / " + d + ".0" + ")"), genType);
+              s := "((" + n + ".0 / " + d + ".0" + ") as " + genType + ")";
             }
           }
 
-          r, resultingOwnership := FromOwned(r, expectedOwnership);
+          isOwned := true;
+          isErased := false;
           readIdents := {};
-          return;
         }
         case Literal(StringLiteral(l)) => {
-          r := R.dafny_runtime.MSel("string_of").Apply1(R.LiteralString(l, false));
-          r, resultingOwnership := FromOwned(r, expectedOwnership);
+          // TODO(shadaj): handle unicode properly
+          s := "\"" + l + "\".chars().collect::<Vec<char>>()";
+          isOwned := true;
+          isErased := false;
           readIdents := {};
-          return;
         }
         case Literal(CharLiteral(c)) => {
-          r := R.LiteralInt(Strings.OfNat(c as nat));
-          if !UnicodeChars {
-            r :=
-              R.global.MSel("std").MSel("primitive")
-              .MSel("char").MSel("from_u16")
-              .Apply1(r).Sel("unwrap").Apply([], []);
-          } else {
-            r :=
-              R.global.MSel("std").MSel("primitive")
-              .MSel("char").MSel("from_u32")
-              .Apply1(r).Sel("unwrap").Apply([], []);
-          }
-          r := R.dafny_runtime.MSel(DafnyChar).Apply1(r);
-          r, resultingOwnership := FromOwned(r, expectedOwnership);
+          s := "::std::primitive::char::from_u32(" + Strings.OfNat(c as nat) + ").unwrap()";
+          isOwned := true;
+          isErased := false;
           readIdents := {};
-          return;
         }
         case Literal(Null(tpe)) => {
-          // TODO: Mikael. Null will be std::ptr::null, not Option::None.
           var tpeGen := GenType(tpe, false, false);
-          r := R.TypeAscription(R.RawExpr("None"), tpeGen);
-          r, resultingOwnership := FromOwned(r, expectedOwnership);
+          s := "(None as " + tpeGen + ")";
+          isOwned := true;
+          isErased := false;
           readIdents := {};
-          return;
         }
-      }
-    }
-
-    method GenExprBinary(
-      e: Expression,
-      selfIdent: Option<string>,
-      params: seq<string>,
-      expectedOwnership: Ownership
-    ) returns (r: R.Expr, resultingOwnership: Ownership, readIdents: set<string>)
-      requires e.BinOp?
-      ensures OwnershipGuarantee(expectedOwnership, resultingOwnership)
-      decreases e, 0
-    {
-      var BinOp(op, lExpr, rExpr, format) := e;
-      var becomesLeftCallsRight := match op {
-        case SetMerge()
-          | SetSubtraction()
-          | SetIntersection()
-          | SetDisjoint()
-          | MapMerge()
-          | MapSubtraction()
-          | MultisetMerge()
-          | MultisetSubtraction()
-          | MultisetIntersection()
-          | MultisetDisjoint()
-          | Concat()
-          => true
-        case _ => false
-      };
-      var becomesRightCallsLeft := match op {
-        case In() => true
-        case _ => false
-      };
-      var becomesCallLeftRight := match op {
-        case Eq(true, false) => true
-        case _ => false
-      };
-      var expectedLeftOwnership :=
-        if becomesLeftCallsRight then OwnershipAutoBorrowed
-        else if becomesRightCallsLeft || becomesCallLeftRight then OwnershipBorrowed
-        else OwnershipOwned;
-      var expectedRightOwnership :=
-        if becomesLeftCallsRight || becomesCallLeftRight then OwnershipBorrowed
-        else if becomesRightCallsLeft then OwnershipAutoBorrowed
-        else OwnershipOwned;
-      var left, _, recIdentsL := GenExpr(lExpr, selfIdent, params, expectedLeftOwnership);
-      var right, _, recIdentsR := GenExpr(rExpr, selfIdent, params, expectedRightOwnership);
-
-      match op {
-        case In() => {
-          r := right.Sel("contains").Apply1(left);
-        }
-        case SeqProperPrefix() =>
-          r := R.BinaryOp("<", left, right, format);
-        case SeqPrefix() =>
-          r := R.BinaryOp("<=", left, right, format);
-        case SetMerge() => {
-          r := left.Sel("merge").Apply1(right);
-        }
-        case SetSubtraction() => {
-          r := left.Sel("subtract").Apply1(right);
-        }
-        case SetIntersection() => {
-          r := left.Sel("intersect").Apply1(right);
-        }
-        case Subset() => {
-          r := R.BinaryOp("<=", left, right, format);
-        }
-        case ProperSubset() => {
-          r := R.BinaryOp("<", left, right, format);
-        }
-        case SetDisjoint() => {
-          r := left.Sel("disjoint").Apply1(right);
-        }
-        case MapMerge() => {
-          r := left.Sel("merge").Apply1(right);
-        }
-        case MapSubtraction() => {
-          r := left.Sel("subtract").Apply1(right);
-        }
-        case MultisetMerge() => {
-          r := left.Sel("merge").Apply1(right);
-        }
-        case MultisetSubtraction() => {
-          r := left.Sel("subtract").Apply1(right);
-        }
-        case MultisetIntersection() => {
-          r := left.Sel("intersect").Apply1(right);
-        }
-        case Submultiset() => {
-          r := R.BinaryOp("<=", left, right, format);
-        }
-        case ProperSubmultiset() => {
-          r := R.BinaryOp("<", left, right, format);
-        }
-        case MultisetDisjoint() => {
-          r := left.Sel("disjoint").Apply1(right);
-        }
-        case Concat() => {
-          r := left.Sel("concat").Apply1(right);
-        }
-        case _ => {
-
-          if op in OpTable {
-            r := R.Expr.BinaryOp(
-              OpTable[op],
-              left,
-              right,
-              format);
-          } else {
-            match op {
-              case Eq(referential, nullable) => {
-                if (referential) {
-                  // TODO: Render using a call with two expressions
-                  if (nullable) {
-                    r := R.Call(R.RawExpr("::dafny_runtime::nullable_referential_equality"), [], [left, right]);
-                  } else {
-                    r := R.Call(R.RawExpr("::std::rc::Rc::ptr_eq"), [], [left, right]);
-                  }
-                } else {
-                  r := R.BinaryOp("==", left, right, DAST.Format.BinaryOpFormat.NoFormat());
-                }
-              }
-              case EuclidianDiv() => {
-                r := R.Call(R.RawExpr("::dafny_runtime::euclidian_division"), [], [left, right]);
-              }
-              case EuclidianMod() => {
-                r := R.Call(R.RawExpr("::dafny_runtime::euclidian_modulo"), [], [left, right]);
-              }
-              case Passthrough(op) => {
-                r := R.Expr.BinaryOp(op, left, right, format);
-              }
-            }
-          }
-        }
-      }
-      r, resultingOwnership := FromOwned(r, expectedOwnership);
-      readIdents := recIdentsL + recIdentsR;
-      return;
-    }
-
-    method GenExprConvertFromNullable(
-      e: Expression,
-      selfIdent: Option<string>,
-      params: seq<string>,
-      expectedOwnership: Ownership
-    ) returns (r: R.Expr, resultingOwnership: Ownership, readIdents: set<string>)
-      requires e.Convert?
-      requires e.from != e.typ
-      requires e.from.Nullable?
-      ensures OwnershipGuarantee(expectedOwnership, resultingOwnership)
-      decreases e, 0, 0
-    {
-      var Convert(expr, fromTpe, toTpe) := e;
-      var recursiveGen, recOwned, recIdents := GenExpr(expr, selfIdent, params, expectedOwnership);
-      r := recursiveGen;
-      if recOwned == OwnershipOwned {
-        r := r.Sel("as_ref").Apply([], []);
-      }
-      r := r.Sel("unwrap").Apply([], []);
-      r, resultingOwnership := FromOwnership(r, recOwned, expectedOwnership);
-      readIdents := recIdents;
-    }
-
-    method GenExprConvertToNullable(
-      e: Expression,
-      selfIdent: Option<string>,
-      params: seq<string>,
-      expectedOwnership: Ownership
-    ) returns (r: R.Expr, resultingOwnership: Ownership, readIdents: set<string>)
-      requires e.Convert?
-      requires e.from != e.typ
-      requires !e.from.Nullable? && e.typ.Nullable?
-      ensures OwnershipGuarantee(expectedOwnership, resultingOwnership)
-      decreases e, 0, 0
-    {
-      var Convert(expr, fromTpe, toTpe) := e;
-      var recursiveGen, recOwned, recIdents := GenExpr(expr, selfIdent, params, expectedOwnership);
-      r := recursiveGen;
-      if recOwned == OwnershipOwned {
-        r := r.Sel("clone").Apply([], []);
-      }
-
-      r := R.std.MSel("option").MSel("Option").MSel("Some").Apply([], [r]);
-      r, resultingOwnership := FromOwnership(r, recOwned, expectedOwnership);
-      readIdents := recIdents;
-    }
-
-    method GenExprConvertToNewtype(
-      e: Expression,
-      selfIdent: Option<string>,
-      params: seq<string>,
-      expectedOwnership: Ownership
-    ) returns (r: R.Expr, resultingOwnership: Ownership, readIdents: set<string>)
-      requires e.Convert?
-      requires e.from != e.typ
-      requires !e.from.Nullable? && e.typ.Path? && e.typ.resolved.Newtype?
-      ensures OwnershipGuarantee(expectedOwnership, resultingOwnership)
-      decreases e, 0, 0
-    {
-      var Convert(expr, fromTpe, toTpe) := e;
-      var Path(_, _, Newtype(b, range, erase)) := toTpe;
-      if fromTpe == b {
-        var recursiveGen, recOwned, recIdents := GenExpr(expr, selfIdent, params, expectedOwnership);
-
-        var potentialRhsType := NewtypeToRustType(b, range);
-        match potentialRhsType {
-          case Some(v) =>
-            r := R.ConversionNum(v, recursiveGen);
-            r, resultingOwnership := FromOwned(r, expectedOwnership);
-          case None =>
-            if erase {
-              r := recursiveGen;
-            } else {
-              var rhsType := GenType(toTpe, true, false);
-              r := R.RawExpr(rhsType.ToString(IND) + "(" + recursiveGen.ToString(IND) + ")");
-            }
-            r, resultingOwnership := FromOwnership(r, recOwned, expectedOwnership);
-        }
-        readIdents := recIdents;
-        assert OwnershipGuarantee(expectedOwnership, resultingOwnership);
-      } else {
-        assume {:axiom} Convert(Convert(expr, fromTpe, b), b, toTpe) < e; // make termination go through
-        r, resultingOwnership, readIdents := GenExpr(Convert(Convert(expr, fromTpe, b), b, toTpe), selfIdent, params, expectedOwnership);
-        assert OwnershipGuarantee(expectedOwnership, resultingOwnership);
-      }
-    }
-
-
-    method GenExprConvertFromNewtype(
-      e: Expression,
-      selfIdent: Option<string>,
-      params: seq<string>,
-      expectedOwnership: Ownership
-    ) returns (r: R.Expr, resultingOwnership: Ownership, readIdents: set<string>)
-      requires e.Convert?
-      requires e.from != e.typ
-      requires !e.from.Nullable? && (!e.typ.Path? || !e.typ.resolved.Newtype?)
-      requires e.from.Path? && e.from.resolved.Newtype?
-      ensures OwnershipGuarantee(expectedOwnership, resultingOwnership)
-      decreases e, 0, 0
-    {
-      var Convert(expr, fromTpe, toTpe) := e;
-      var Path(_, _, Newtype(b, range, erase)) := fromTpe;
-      if b == toTpe {
-        var recursiveGen, recOwned, recIdents := GenExpr(expr, selfIdent, params, expectedOwnership);
-        if erase {
-          r := recursiveGen;
-        } else {
-          r := recursiveGen.Sel("0");
-        }
-        r, resultingOwnership := FromOwnership(r, recOwned, expectedOwnership);
-        readIdents := recIdents;
-      } else {
-        assume {:axiom} Convert(Convert(expr, fromTpe, b), b, toTpe) < e; // make termination go through
-        r, resultingOwnership, readIdents := GenExpr(Convert(Convert(expr, fromTpe, b), b, toTpe), selfIdent, params, expectedOwnership);
-      }
-      assert OwnershipGuarantee(expectedOwnership, resultingOwnership);
-    }
-
-    method GenExprConvertNotImplemented(
-      e: Expression,
-      selfIdent: Option<string>,
-      params: seq<string>,
-      expectedOwnership: Ownership
-    ) returns (r: R.Expr, resultingOwnership: Ownership, readIdents: set<string>)
-      requires e.Convert?
-      ensures OwnershipGuarantee(expectedOwnership, resultingOwnership)
-      decreases e, 0, 0
-    {
-      var Convert(expr, fromTpe, toTpe) := e;
-      var recursiveGen, recOwned, recIdents := GenExpr(expr, selfIdent, params, expectedOwnership);
-      r := R.RawExpr("(" + recursiveGen.ToString(IND) + "/* conversion not yet implemented */)");
-      r, resultingOwnership := FromOwned(r, expectedOwnership);
-      readIdents := recIdents;
-    }
-
-    method GenExprConvert(
-      e: Expression,
-      selfIdent: Option<string>,
-      params: seq<string>,
-      expectedOwnership: Ownership
-    ) returns (r: R.Expr, resultingOwnership: Ownership, readIdents: set<string>)
-      requires e.Convert?
-      ensures OwnershipGuarantee(expectedOwnership, resultingOwnership)
-      decreases e, 0
-    {
-      var Convert(expr, fromTpe, toTpe) := e;
-      if fromTpe == toTpe {
-        var recursiveGen, recOwned, recIdents := GenExpr(expr, selfIdent, params, expectedOwnership);
-        r := recursiveGen;
-        r, resultingOwnership := FromOwnership(r, recOwned, expectedOwnership);
-        readIdents := recIdents;
-      } else {
-        match (fromTpe, toTpe) {
-          case (Nullable(_), _) => {
-            r, resultingOwnership, readIdents := GenExprConvertFromNullable(e, selfIdent, params, expectedOwnership);
-          }
-          case (_, Nullable(_)) => {
-            r, resultingOwnership, readIdents := GenExprConvertToNullable(e, selfIdent, params, expectedOwnership);
-          }
-          case (_, Path(_, _, Newtype(b, range, erase))) => {
-            r, resultingOwnership, readIdents := GenExprConvertToNewtype(e, selfIdent, params, expectedOwnership);
-          }
-          case (Path(_, _, Newtype(b, range, erase)), _) => {
-            r, resultingOwnership, readIdents := GenExprConvertFromNewtype(e, selfIdent, params, expectedOwnership);
-          }
-          case (Primitive(Int), Primitive(Real)) => {
-            var recursiveGen, _, recIdents := GenExpr(expr, selfIdent, params, OwnershipOwned);
-            r := R.RcNew(R.RawExpr("::dafny_runtime::BigRational::from_integer(" + recursiveGen.ToString(IND) + ")"));
-            r, resultingOwnership := FromOwned(r, expectedOwnership);
-            readIdents := recIdents;
-          }
-          case (Primitive(Real), Primitive(Int)) => {
-            var recursiveGen, _, recIdents := GenExpr(expr, selfIdent, params, OwnershipBorrowed);
-            r := R.RawExpr("::dafny_runtime::dafny_rational_to_int(" + recursiveGen.ToString(IND) + ")");
-            r, resultingOwnership := FromOwned(r, expectedOwnership);
-            readIdents := recIdents;
-          }
-          case (Primitive(Int), Passthrough(_)) => {
-            var rhsType := GenType(toTpe, true, false);
-            var recursiveGen, _, recIdents := GenExpr(expr, selfIdent, params, OwnershipOwned);
-            r := R.RawExpr("<" + rhsType.ToString(IND) + " as ::dafny_runtime::NumCast>::from(" + recursiveGen.ToString(IND) + ").unwrap()");
-            r, resultingOwnership := FromOwned(r, expectedOwnership);
-            readIdents := recIdents;
-          }
-          case (Passthrough(_), Primitive(Int)) => {
-            var rhsType := GenType(fromTpe, true, false);
-            var recursiveGen, _, recIdents := GenExpr(expr, selfIdent, params, OwnershipOwned);
-            r := R.RawExpr("::dafny_runtime::DafnyInt{data: ::dafny_runtime::BigInt::from(" + recursiveGen.ToString(IND) + ")}");
-            r, resultingOwnership := FromOwned(r, expectedOwnership);
-            readIdents := recIdents;
-          }
-          case (Primitive(Int), Primitive(Char)) => {
-            var rhsType := GenType(toTpe, true, false);
-            var recursiveGen, _, recIdents := GenExpr(expr, selfIdent, params, OwnershipOwned);
-            r := R.RawExpr("char::from_u32(<u32 as ::dafny_runtime::NumCast>::from(" + recursiveGen.ToString(IND) + ").unwrap()).unwrap()");
-            r, resultingOwnership := FromOwned(r, expectedOwnership);
-            readIdents := recIdents;
-          }
-          case (Primitive(Char), Primitive(Int)) => {
-            var rhsType := GenType(fromTpe, true, false);
-            var recursiveGen, _, recIdents := GenExpr(expr, selfIdent, params, OwnershipOwned);
-            r := R.RawExpr("::dafny_runtime::DafnyInt{data: ::BigInt::from(" + recursiveGen.ToString(IND) + " as u32)}");
-            r, resultingOwnership := FromOwned(r, expectedOwnership);
-            readIdents := recIdents;
-          }
-          case (Passthrough(_), Passthrough(_)) => {
-            var recursiveGen, _, recIdents := GenExpr(expr, selfIdent, params, OwnershipOwned);
-            var toTpeGen := GenType(toTpe, true, false);
-
-            r := R.RawExpr("((" + recursiveGen.ToString(IND) + ") as " + toTpeGen.ToString(IND) + ")");
-
-            r, resultingOwnership := FromOwned(r, expectedOwnership);
-            readIdents := recIdents;
-          }
-          case _ => {
-            r, resultingOwnership, readIdents := GenExprConvertNotImplemented(e, selfIdent, params, expectedOwnership);
-          }
-        }
-      }
-      assert OwnershipGuarantee(expectedOwnership, resultingOwnership);
-      return;
-    }
-    method GenExpr(
-      e: Expression,
-      selfIdent: Option<string>,
-      params: seq<string>,
-      expectedOwnership: Ownership
-    ) returns (r: R.Expr, resultingOwnership: Ownership, readIdents: set<string>)
-      ensures OwnershipGuarantee(expectedOwnership, resultingOwnership)
-      decreases e, 1 {
-      match e {
-        case Literal(_) =>
-          r, resultingOwnership, readIdents :=
-            GenExprLiteral(e, selfIdent, params, expectedOwnership);
         case Ident(name) => {
-          r := R.Identifier(escapeIdent(name));
-          var currentlyBorrowed := name in params; // Otherwise names are owned  // TODO(mikael) have a table to know which names are borrowed
-          if expectedOwnership == OwnershipAutoBorrowed {
-            resultingOwnership := OwnershipOwned;
-            // No need to do anything
-          } else if expectedOwnership == OwnershipBorrowedMut {
-            r := R.BorrowMut(r); // Needs to be explicit for out-parameters on methods
-            resultingOwnership := OwnershipBorrowedMut;
-          } else if expectedOwnership == OwnershipOwned {
-            r := R.Clone(r); // We don't transfer the ownership of an identifier
-            resultingOwnership := OwnershipOwned;
-          } else if currentlyBorrowed {
-            assert expectedOwnership == OwnershipBorrowed;
-            resultingOwnership := OwnershipBorrowed;
-          } else {
-            // It's currently owned.
-            r := R.Borrow(r);
-            resultingOwnership := OwnershipBorrowed;
+          s := escapeIdent(name);
+          if !(name in params) {
+            s := "(&" + s + ")";
           }
+
+          if mustOwn {
+            s := s + ".clone()";
+            isOwned := true;
+          } else {
+            isOwned := false;
+          }
+
+          isErased := false;
+
           readIdents := {name};
-          return;
         }
         case Companion(path) => {
-          var p := GenPath(path);
-          r := R.RawExpr(p);
-          r, resultingOwnership := FromOwned(r, expectedOwnership);
+          s := GenPath(path);
+          isOwned := true;
+          isErased := true;
           readIdents := {};
-          return;
         }
         case InitializationValue(typ) => {
-          var typExpr := GenType(typ, false, false);
-          r := R.RawExpr("<" + typExpr.ToString(IND) + " as std::default::Default>::default()");
-          r, resultingOwnership := FromOwned(r, expectedOwnership);
+          var typString := GenType(typ, false, false);
+          s := "<" + typString + " as std::default::Default>::default()";
+          isOwned := true;
+          isErased := false;
           readIdents := {};
-          return;
         }
         case Tuple(values) => {
-          var s := "(";
+          s := "(";
           readIdents := {};
 
           var i := 0;
@@ -2742,33 +1724,37 @@ module {:extern "DCOMP"} DafnyToRustCompiler {
               s := s + " ";
             }
 
-            var recursiveGen, _, recIdents := GenExpr(values[i], selfIdent, params, OwnershipOwned);
+            var recursiveGen, _, isErased, recIdents := GenExpr(values[i], selfIdent, params, true);
+            if isErased {
+              recursiveGen := "::dafny_runtime::DafnyUnerasable::<_>::unerase_owned(" + recursiveGen + ")";
+            }
 
-            s := s + recursiveGen.ToString(IND) + ",";
+            s := s + recursiveGen + ",";
             readIdents := readIdents + recIdents;
 
             i := i + 1;
           }
           s := s + ")";
-          r := R.RawExpr(s);
-
-          r, resultingOwnership := FromOwned(r, expectedOwnership);
-          return;
+          isOwned := true;
+          isErased := false;
         }
         case New(path, typeArgs, args) => {
           var path := GenPath(path);
-          // TODO(Mikael) Use allocate(...) here.
-          var s := "::std::rc::Rc::new(" + path;
+          s := "::std::rc::Rc::new(" + path;
           if |typeArgs| > 0 {
+            s := s + "::<";
             var i := 0;
-            var typeExprs := [];
             while i < |typeArgs| {
-              var typeExpr := GenType(typeArgs[i], false, false);
-              typeExprs := typeExprs + [typeExpr];
+              if i > 0 {
+                s := s + "::";
+              }
+
+              var typeString := GenType(typeArgs[i], false, false);
+              s := s + typeString;
 
               i := i + 1;
             }
-            s := s + R.TypeApp(R.TIdentifier("::"), typeExprs).ToString(IND);
+            s := s + ">";
           }
           s := s + "::new(";
           readIdents := {};
@@ -2778,39 +1764,42 @@ module {:extern "DCOMP"} DafnyToRustCompiler {
               s := s + ", ";
             }
 
-            var recursiveGen, _, recIdents := GenExpr(args[i], selfIdent, params, OwnershipOwned);
-            s := s + recursiveGen.ToString(IND);
+            var recursiveGen, _, isErased, recIdents := GenExpr(args[i], selfIdent, params, true);
+            if isErased {
+              recursiveGen := "::dafny_runtime::DafnyUnerasable::<_>::unerase_owned(" + recursiveGen + ")";
+            }
+            s := s + recursiveGen;
             readIdents := readIdents + recIdents;
 
             i := i + 1;
           }
           s := s + "))";
-          r := R.RawExpr(s);
-          r, resultingOwnership := FromOwned(r, expectedOwnership);
-          return;
+          isOwned := true;
+          isErased := true;
         }
         case NewArray(dims, typ) => {
           var i := |dims| - 1;
           var genTyp := GenType(typ, false, false);
-          // TODO (Mikael): Prevent arrays from being initialized without initialization code
-          var s := "<" + genTyp.ToString(IND) + " as ::std::default::Default>::default()";
+          s := "<" + genTyp + " as ::std::default::Default>::default()";
           readIdents := {};
           while i >= 0 {
-            var recursiveGen, _, recIdents := GenExpr(dims[i], selfIdent, params, OwnershipOwned);
+            var recursiveGen, _, isErased, recIdents := GenExpr(dims[i], selfIdent, params, true);
+            if !isErased {
+              recursiveGen := "::dafny_runtime::DafnyErasable::erase_owned(" + recursiveGen + ")";
+            }
 
-            s := "::std::rc::Rc::new(::std::cell::RefCell::new(vec![" + s + "; <usize as ::dafny_runtime::NumCast>::from(" + recursiveGen.ToString(IND) + ").unwrap()]))";
+            s := "::std::rc::Rc::new(::std::cell::RefCell::new(vec![" + s + "; <usize as ::dafny_runtime::NumCast>::from(" + recursiveGen + ").unwrap()]))";
             readIdents := readIdents + recIdents;
 
             i := i - 1;
           }
 
-          r := R.RawExpr(s);
-          r, resultingOwnership := FromOwned(r, expectedOwnership);
-          return;
+          isOwned := true;
+          isErased := false;
         }
         case DatatypeValue(path, typeArgs, variant, isCo, values) => {
           var path := GenPath(path);
-          var s := "::std::rc::Rc::new(" + path + "::";
+          s := "::std::rc::Rc::new(" + path + "::";
           if |typeArgs| > 0 {
             s := s + "<";
             var i := 0;
@@ -2819,8 +1808,8 @@ module {:extern "DCOMP"} DafnyToRustCompiler {
                 s := s + ", ";
               }
 
-              var typeExpr := GenType(typeArgs[i], false, false);
-              s := s + typeExpr.ToString(IND);
+              var typeString := GenType(typeArgs[i], false, false);
+              s := s + typeString;
 
               i := i + 1;
             }
@@ -2838,7 +1827,11 @@ module {:extern "DCOMP"} DafnyToRustCompiler {
             }
 
             if isCo {
-              var recursiveGen, _, recIdents := GenExpr(value, selfIdent, [], OwnershipOwned);
+              var recursiveGen, _, isErased, recIdents := GenExpr(value, selfIdent, [], true);
+              if !isErased {
+                recursiveGen := "::dafny_runtime::DafnyErasable::erase_owned(" + recursiveGen + ")";
+              }
+              recursiveGen := "::dafny_runtime::DafnyUnerasable::<_>::unerase_owned(" + recursiveGen + ")";
 
               readIdents := readIdents + recIdents;
               var allReadCloned := "";
@@ -2847,34 +1840,161 @@ module {:extern "DCOMP"} DafnyToRustCompiler {
                 allReadCloned := allReadCloned + "let " + escapeIdent(next) + " = " + escapeIdent(next) + ".clone();\n";
                 recIdents := recIdents - {next};
               }
-              s := s + escapeIdent(name) + ": ::dafny_runtime::LazyFieldWrapper(::dafny_runtime::Lazy::new(::std::boxed::Box::new({\n" + allReadCloned + "move || (" + recursiveGen.ToString(IND) + ")})))";
+              s := s + escapeIdent(name) + ": ::dafny_runtime::LazyFieldWrapper(::dafny_runtime::Lazy::new(::std::boxed::Box::new({\n" + allReadCloned + "move || (" + recursiveGen + ")})))";
             } else {
-              var recursiveGen, _, recIdents := GenExpr(value, selfIdent, params, OwnershipOwned);
+              var recursiveGen, _, isErased, recIdents := GenExpr(value, selfIdent, params, true);
+              if !isErased {
+                recursiveGen := "::dafny_runtime::DafnyErasable::erase_owned(" + recursiveGen + ")";
+              }
+              recursiveGen := "::dafny_runtime::DafnyUnerasable::<_>::unerase_owned(" + recursiveGen + ")";
 
-              s := s + escapeIdent(name) + ": " + "(" + recursiveGen.ToString(IND) + ")";
+              s := s + escapeIdent(name) + ": " + "(" + recursiveGen + ")";
               readIdents := readIdents + recIdents;
             }
             i := i + 1;
           }
           s := s + " })";
-
-          r := R.RawExpr(s);
-          r, resultingOwnership := FromOwned(r, expectedOwnership);
-          return;
+          isOwned := true;
+          isErased := false;
         }
-        case Convert(_, _, _) => {
-          r, resultingOwnership, readIdents :=
-            GenExprConvert(e, selfIdent, params, expectedOwnership);
+        case Convert(expr, fromTpe, toTpe) => {
+          if fromTpe == toTpe {
+            var recursiveGen, recOwned, recErased, recIdents := GenExpr(expr, selfIdent, params, mustOwn);
+            s := recursiveGen;
+            isOwned := recOwned;
+            isErased := recErased;
+            readIdents := recIdents;
+          } else {
+            match (fromTpe, toTpe) {
+              case (Nullable(_), _) => {
+                var recursiveGen, recOwned, recErased, recIdents := GenExpr(expr, selfIdent, params, mustOwn);
+                if !recOwned {
+                  recursiveGen := recursiveGen + ".as_ref()";
+                }
+
+                s := recursiveGen + ".unwrap()";
+                isOwned := recOwned;
+                isErased := recErased;
+                readIdents := recIdents;
+              }
+              case (_, Nullable(_)) => {
+                var recursiveGen, recOwned, recErased, recIdents := GenExpr(expr, selfIdent, params, mustOwn);
+                if !recOwned {
+                  recursiveGen := recursiveGen + ".clone()";
+                }
+
+                s := "Some(" + recursiveGen + ")";
+                isOwned := true;
+                isErased := recErased;
+                readIdents := recIdents;
+              }
+              case (_, Path(_, _, Newtype(b))) => {
+                if fromTpe == b {
+                  var recursiveGen, recOwned, recErased, recIdents := GenExpr(expr, selfIdent, params, mustOwn);
+
+                  var rhsType := GenType(toTpe, true, false);
+
+                  var uneraseFn := if recOwned then "unerase_owned" else "unerase";
+                  s := "<" + rhsType + " as ::dafny_runtime::DafnyUnerasable<_>>::" + uneraseFn + "(" + recursiveGen + ")";
+                  isOwned := recOwned;
+                  isErased := false;
+                  readIdents := recIdents;
+                } else {
+                  assume {:axiom} Convert(Convert(expr, fromTpe, b), b, toTpe) < e; // make termination go through
+                  s, isOwned, isErased, readIdents := GenExpr(Convert(Convert(expr, fromTpe, b), b, toTpe), selfIdent, params, mustOwn);
+                }
+              }
+              case (Path(_, _, Newtype(b)), _) => {
+                if b == toTpe {
+                  var recursiveGen, recOwned, recErased, recIdents := GenExpr(expr, selfIdent, params, mustOwn);
+                  var uneraseFn := if recOwned then "erase_owned" else "erase";
+                  s := "::dafny_runtime::DafnyErasable::" + uneraseFn + "(" + recursiveGen + ")";
+                  isOwned := recOwned;
+                  isErased := true;
+                  readIdents := recIdents;
+                } else {
+                  assume {:axiom} Convert(Convert(expr, fromTpe, b), b, toTpe) < e; // make termination go through
+                  s, isOwned, isErased, readIdents := GenExpr(Convert(Convert(expr, fromTpe, b), b, toTpe), selfIdent, params, mustOwn);
+                }
+              }
+              case (Primitive(Int), Primitive(Real)) => {
+                var recursiveGen, _, _, recIdents := GenExpr(expr, selfIdent, params, true);
+                s := "::dafny_runtime::BigRational::from_integer(" + recursiveGen + ")";
+                isOwned := true;
+                isErased := true;
+                readIdents := recIdents;
+              }
+              case (Primitive(Real), Primitive(Int)) => {
+                var recursiveGen, _, _, recIdents := GenExpr(expr, selfIdent, params, false);
+                s := "::dafny_runtime::dafny_rational_to_int(" + recursiveGen + ")";
+                isOwned := true;
+                isErased := true;
+                readIdents := recIdents;
+              }
+              case (Primitive(Int), Passthrough(_)) => {
+                var rhsType := GenType(toTpe, true, false);
+                var recursiveGen, _, _, recIdents := GenExpr(expr, selfIdent, params, true);
+                s := "<" + rhsType + " as ::dafny_runtime::NumCast>::from(" + recursiveGen + ").unwrap()";
+                isOwned := true;
+                isErased := true;
+                readIdents := recIdents;
+              }
+              case (Passthrough(_), Primitive(Int)) => {
+                var rhsType := GenType(fromTpe, true, false);
+                var recursiveGen, _, _, recIdents := GenExpr(expr, selfIdent, params, true);
+                s := "::dafny_runtime::BigInt::from(" + recursiveGen + ")";
+                isOwned := true;
+                isErased := true;
+                readIdents := recIdents;
+              }
+              case (Primitive(Int), Primitive(Char)) => {
+                var rhsType := GenType(toTpe, true, false);
+                var recursiveGen, _, _, recIdents := GenExpr(expr, selfIdent, params, true);
+                s := "char::from_u32(<u32 as ::dafny_runtime::NumCast>::from(" + recursiveGen + ").unwrap()).unwrap()";
+                isOwned := true;
+                isErased := true;
+                readIdents := recIdents;
+              }
+              case (Primitive(Char), Primitive(Int)) => {
+                var rhsType := GenType(fromTpe, true, false);
+                var recursiveGen, _, _, recIdents := GenExpr(expr, selfIdent, params, true);
+                s := "::dafny_runtime::BigInt::from(" + recursiveGen + " as u32)";
+                isOwned := true;
+                isErased := true;
+                readIdents := recIdents;
+              }
+              case (Passthrough(_), Passthrough(_)) => {
+                var recursiveGen, _, _, recIdents := GenExpr(expr, selfIdent, params, true);
+                var toTpeGen := GenType(toTpe, true, false);
+
+                s := "((" + recursiveGen + ") as " + toTpeGen + ")";
+
+                isOwned := true;
+                isErased := true;
+                readIdents := recIdents;
+              }
+              case _ => {
+                var recursiveGen, recOwned, recErased, recIdents := GenExpr(expr, selfIdent, params, mustOwn);
+                s := "(" + recursiveGen + "/* conversion not yet implemented */)";
+                isOwned := recOwned;
+                isErased := recErased;
+                readIdents := recIdents;
+              }
+            }
+          }
         }
         case SeqConstruct(length, expr) => {
-          var recursiveGen, _, recIdents := GenExpr(expr, selfIdent, params, OwnershipOwned);
-          var lengthGen, _, lengthIdents := GenExpr(length, selfIdent, params, OwnershipOwned);
+          var recursiveGen, _, eErased, recIdents := GenExpr(expr, selfIdent, params, true);
+          var lengthGen, _, lengthErased, lengthIdents := GenExpr(length, selfIdent, params, true);
+          if !lengthErased {
+            lengthGen := "::dafny_runtime::DafnyErasable::erase_owned(" + lengthGen + ")";
+          }
 
-          r := R.RawExpr("{\nlet _initializer = " + recursiveGen.ToString(IND) + ";\n::dafny_runtime::integer_range(::dafny_runtime::Zero::zero(), " + lengthGen.ToString(IND) + ").map(|i| _initializer.0(&i)).collect::<::dafny_runtime::Sequence<_>>()\n}");
+          s := "{\nlet _initializer = " + recursiveGen + ";\n::dafny_runtime::integer_range(::dafny_runtime::Zero::zero(), " + lengthGen + ").map(|i| _initializer.0(&i)).collect::<Vec<_>>()\n}";
 
           readIdents := recIdents + lengthIdents;
-          r, resultingOwnership := FromOwned(r, expectedOwnership);
-          return;
+          isOwned := true;
+          isErased := eErased;
         }
         case SeqValue(exprs, typ) => {
           readIdents := {};
@@ -2882,222 +2002,295 @@ module {:extern "DCOMP"} DafnyToRustCompiler {
           var genTpe := GenType(typ, false, false);
 
           var i := 0;
-          var args := [];
+          s := "(vec![";
+          i := 0;
           while i < |exprs| {
-            var recursiveGen, _, recIdents := GenExpr(exprs[i], selfIdent, params, OwnershipOwned);
-            readIdents := readIdents + recIdents;
-            args := args + [recursiveGen];
+            if i > 0 {
+              s := s + ", ";
+            }
 
+            var recursiveGen, _, isErased, recIdents := GenExpr(exprs[i], selfIdent, params, true);
+            readIdents := readIdents + recIdents;
+
+            if isErased {
+              recursiveGen := "::dafny_runtime::DafnyUnerasable::<_>::unerase_owned(" + recursiveGen + ")";
+            }
+
+            s := s + recursiveGen;
             i := i + 1;
           }
-          r := R.dafny_runtime.MSel("seq!").Apply([], args);
-          if |args| == 0 {
-            r := R.TypeAscription(r,
-                                  R.dafny_runtime_type.MSel("Sequence").Apply1(genTpe));
-          }
-          r, resultingOwnership := FromOwned(r, expectedOwnership);
-          return;
+          s := s + "] as Vec<" + genTpe + ">)";
+
+          isOwned := true;
+          isErased := false;
         }
         case SetValue(exprs) => {
           var generatedValues := [];
           readIdents := {};
           var i := 0;
+          var allErased := true;
           while i < |exprs| {
-            var recursiveGen, _, recIdents := GenExpr(exprs[i], selfIdent, params, OwnershipOwned);
+            var recursiveGen, _, isErased, recIdents := GenExpr(exprs[i], selfIdent, params, true);
+            allErased := allErased && isErased;
 
-            generatedValues := generatedValues + [recursiveGen];
+            generatedValues := generatedValues + [(recursiveGen, isErased)];
             readIdents := readIdents + recIdents;
             i := i + 1;
           }
-          r := R.dafny_runtime.MSel("set!").Apply([], generatedValues);
-          r, resultingOwnership := FromOwned(r, expectedOwnership);
-          return;
-        }
-        case MultisetValue(exprs) => {
-          var generatedValues := [];
-          readIdents := {};
-          var i := 0;
-          while i < |exprs| {
-            var recursiveGen, _, recIdents := GenExpr(exprs[i], selfIdent, params, OwnershipOwned);
 
-            generatedValues := generatedValues + [recursiveGen];
-            readIdents := readIdents + recIdents;
+          s := "vec![";
+          i := 0;
+          while i < |generatedValues| {
+            if i > 0 {
+              s := s + ", ";
+            }
+
+            var gen := generatedValues[i].0;
+            if generatedValues[i].1 && !allErased {
+              gen := "::dafny_runtime::DafnyUnerasable::<_>::unerase_owned(" + gen + ")";
+            }
+
+            s := s + gen;
             i := i + 1;
           }
-          r := R.dafny_runtime.MSel("multiset!").Apply([], generatedValues);
-          r, resultingOwnership := FromOwned(r, expectedOwnership);
-          return;
-        }
-        case ToMultiset(expr) => {
-          var recursiveGen, _, recIdents := GenExpr(expr, selfIdent, params, OwnershipAutoBorrowed);
-          r := recursiveGen.Sel("as_dafny_multiset").Apply([], []);
-          readIdents := recIdents;
-          r, resultingOwnership := FromOwned(r, expectedOwnership);
-          return;
+          s := s + "].into_iter().collect::<std::collections::HashSet<_>>()";
+
+          isOwned := true;
+          isErased := allErased;
         }
         case MapValue(mapElems) => {
           var generatedValues := [];
           readIdents := {};
           var i := 0;
+          var allErased := true;
           while i < |mapElems| {
-            var recursiveGenKey, _, recIdentsKey := GenExpr(mapElems[i].0, selfIdent, params, OwnershipOwned);
-            var recursiveGenValue, _, recIdentsValue := GenExpr(mapElems[i].1, selfIdent, params, OwnershipOwned);
+            var recursiveGenKey, _, isErasedKey, recIdentsKey := GenExpr(mapElems[i].0, selfIdent, params, true);
+            var recursiveGenValue, _, isErasedValue, recIdentsValue := GenExpr(mapElems[i].1, selfIdent, params, true);
+            allErased := allErased && isErasedKey && isErasedValue;
 
-            generatedValues := generatedValues + [(recursiveGenKey, recursiveGenValue)];
+            generatedValues := generatedValues + [(recursiveGenKey, recursiveGenValue, isErasedKey, isErasedValue)];
             readIdents := readIdents + recIdentsKey + recIdentsValue;
             i := i + 1;
           }
 
+          s := "vec![";
           i := 0;
-          var arguments := [];
           while i < |generatedValues| {
+            if i > 0 {
+              s := s + ", ";
+            }
+
             var genKey := generatedValues[i].0;
             var genValue := generatedValues[i].1;
+            if generatedValues[i].2 && !allErased {
+              genKey := "::dafny_runtime::DafnyUnerasable::<_>::unerase_owned(" + genKey + ")";
+            }
+            if generatedValues[i].3 && !allErased {
+              genValue := "::dafny_runtime::DafnyUnerasable::<_>::unerase_owned(" + genValue + ")";
+            }
 
-            arguments := arguments + [R.BinaryOp("=>", genKey, genValue, DAST.Format.BinaryOpFormat.NoFormat())];
+            s := s + "(" + genKey + ", " + genValue + ")";
             i := i + 1;
           }
-          r := R.dafny_runtime.MSel("map!").Apply([],
-                                                  arguments
-          );
-          r, resultingOwnership := FromOwned(r, expectedOwnership);
-          return;
-        }
-        case SeqUpdate(expr, index, value) => {
-          var exprR, _, exprIdents := GenExpr(expr, selfIdent, params, OwnershipAutoBorrowed);
-          var indexR, indexOwnership, indexIdents := GenExpr(index, selfIdent, params, OwnershipBorrowed);
-          var valueR, valueOwnership, valueIdents := GenExpr(value, selfIdent, params, OwnershipBorrowed);
-          r := exprR.Sel("update_index").Apply([], [indexR, valueR]);
-          r, resultingOwnership := FromOwned(r, expectedOwnership);
-          readIdents := exprIdents + indexIdents + valueIdents;
-          return;
-        }
-        case MapUpdate(expr, index, value) => {
-          var exprR, _, exprIdents := GenExpr(expr, selfIdent, params, OwnershipAutoBorrowed);
-          var indexR, indexOwnership, indexIdents := GenExpr(index, selfIdent, params, OwnershipBorrowed);
-          var valueR, valueOwnership, valueIdents := GenExpr(value, selfIdent, params, OwnershipBorrowed);
-          r := exprR.Sel("update_index").Apply([], [indexR, valueR]);
-          r, resultingOwnership := FromOwned(r, expectedOwnership);
-          readIdents := exprIdents + indexIdents + valueIdents;
-          return;
+          s := s + "].into_iter().collect::<std::collections::HashMap<_, _>>()";
+
+          isOwned := true;
+          isErased := allErased;
         }
         case This() => {
           match selfIdent {
             case Some(id) => {
-              r := R.RawExpr(id);
-              if expectedOwnership == OwnershipOwned {
-                r := R.Clone(r);
-                resultingOwnership := OwnershipOwned;
-              } else if expectedOwnership == OwnershipBorrowed || expectedOwnership == OwnershipAutoBorrowed {
-                if id != "self" {
-                  r := R.Borrow(r);
-                }
-                resultingOwnership := OwnershipBorrowed;
+              if mustOwn {
+                s := id + ".clone()";
+                isOwned := true;
               } else {
-                assert expectedOwnership == OwnershipBorrowedMut;
-                if id != "self" {
-                  r := R.BorrowMut(r);
+                if id == "self" {
+                  s := "self";
+                } else {
+                  s := "&" + id;
                 }
-                resultingOwnership := OwnershipBorrowedMut;
+                isOwned := false;
               }
 
               readIdents := {id};
+              isErased := false;
             }
             case None => {
-              r := R.RawExpr("panic!(\"this outside of a method\")");
-              r, resultingOwnership := FromOwned(r, expectedOwnership);
+              s := "panic!(\"this outside of a method\")";
+              isOwned := true;
               readIdents := {};
+              isErased := true;
             }
           }
-          return;
         }
         case Ite(cond, t, f) => {
-          assert {:split_here} true;
-          var cond, _, recIdentsCond := GenExpr(cond, selfIdent, params, OwnershipOwned);
-          var condString := cond.ToString(IND);
+          var condString, _, condErased, recIdentsCond := GenExpr(cond, selfIdent, params, true);
+          if !condErased {
+            condString := "::dafny_runtime::DafnyErasable::erase_owned(" + condString + ")";
+          }
 
-          var _, tHasToBeOwned, _ := GenExpr(t, selfIdent, params, expectedOwnership); // check if t has to be owned even if not requested
-          var fExpr, fOwned, recIdentsF := GenExpr(f, selfIdent, params, tHasToBeOwned);
-          var fString := fExpr.ToString(IND);
-          var tExpr, _, recIdentsT := GenExpr(t, selfIdent, params, fOwned); // there's a chance that f forced ownership
-          var tString := tExpr.ToString(IND);
+          var _, tHasToBeOwned, _, _ := GenExpr(t, selfIdent, params, mustOwn); // check if t has to be owned even if not requested
+          var fString, fOwned, fErased, recIdentsF := GenExpr(f, selfIdent, params, tHasToBeOwned);
+          var tString, _, tErased, recIdentsT := GenExpr(t, selfIdent, params, fOwned); // there's a chance that f forced ownership
 
-          r := R.RawExpr("(if " + condString + " {\n" + tString + "\n} else {\n" + fString + "\n})");
+          if !fErased || !tErased {
+            if fErased {
+              fString := "::dafny_runtime::DafnyErasable::erase_owned(" + fString + ")";
+            }
 
-          r, resultingOwnership := FromOwnership(r, fOwned, expectedOwnership);
+            if tErased {
+              tString := "::dafny_runtime::DafnyErasable::erase_owned(" + tString + ")";
+            }
+          }
+
+          s := "(if " + condString + " {\n" + tString + "\n} else {\n" + fString + "\n})";
+          isOwned := fOwned;
           readIdents := recIdentsCond + recIdentsT + recIdentsF;
-          return;
+          isErased := fErased || tErased;
         }
-        case UnOp(Not, e, format) => {
-          var recursiveGen, _, recIdents := GenExpr(e, selfIdent, params, OwnershipOwned);
+        case UnOp(Not, e) => {
+          var recursiveGen, _, recErased, recIdents := GenExpr(e, selfIdent, params, true);
+          if !recErased {
+            recursiveGen := "::dafny_runtime::DafnyErasable::erase_owned(" + recursiveGen + ")";
+          }
 
-          r := R.UnaryOp("!", recursiveGen, format);
-          r, resultingOwnership := FromOwned(r, expectedOwnership);
+          s := "!(" + recursiveGen + ")";
+          isOwned := true;
           readIdents := recIdents;
-          return;
+          isErased := true;
         }
-        case UnOp(BitwiseNot, e, format) => {
-          var recursiveGen, _, recIdents := GenExpr(e, selfIdent, params, OwnershipOwned);
+        case UnOp(BitwiseNot, e) => {
+          var recursiveGen, _, recErased, recIdents := GenExpr(e, selfIdent, params, true);
+          if !recErased {
+            recursiveGen := "::dafny_runtime::DafnyErasable::erase_owned(" + recursiveGen + ")";
+          }
 
-          r := R.UnaryOp("~", recursiveGen, format);
-          r, resultingOwnership := FromOwned(r, expectedOwnership);
+          s := "~(" + recursiveGen + ")";
+          isOwned := true;
           readIdents := recIdents;
-          return;
+          isErased := true;
         }
-        case UnOp(Cardinality, e, format) => {
-          var recursiveGen, recOwned, recIdents := GenExpr(e, selfIdent, params, OwnershipAutoBorrowed);
+        case UnOp(Cardinality, e) => {
+          var recursiveGen, recOwned, recErased, recIdents := GenExpr(e, selfIdent, params, false);
+          if !recErased {
+            var eraseFn := if recOwned then "erase_owned" else "erase";
+            recursiveGen := "::dafny_runtime::DafnyErasable::" + eraseFn + "(" + recursiveGen + ")";
+          }
 
-          r := recursiveGen.Sel("cardinality").Apply([], []);
-          r, resultingOwnership := FromOwned(r, expectedOwnership);
+          s := "::dafny_runtime::BigInt::from((" + recursiveGen + ").len())";
+          isOwned := true;
           readIdents := recIdents;
-          return;
+          isErased := true;
         }
-        case BinOp(_, _, _, _) =>
-          r, resultingOwnership, readIdents :=
-            GenExprBinary(e, selfIdent, params, expectedOwnership);
+        case BinOp(op, l, r) => {
+          var left, _, leftErased, recIdentsL := GenExpr(l, selfIdent, params, true);
+          var right, _, rightErased, recIdentsR := GenExpr(r, selfIdent, params, true);
+
+          match op {
+            case Implies() => {
+              if !leftErased {
+                left := "::dafny_runtime::DafnyErasable::erase_owned(" + left + ")";
+              }
+              if !rightErased {
+                right := "::dafny_runtime::DafnyErasable::erase_owned(" + right + ")";
+              }
+              s := "!(" + left + ") || " + right;
+            }
+            case In() => {
+              s := right + ".contains(&" + left + ")";
+            }
+            case NotIn() => {
+              s := "!(" + right + ".contains(&" + left + "))";
+            }
+            case SetDifference() => {
+              s := left + ".difference(&" + right + ").cloned().collect::<::std::collections::HashSet<_>>()";
+            }
+            case Concat() => {
+              s := "[" + left + ", " + right + "].concat()";
+            }
+            case _ => {
+              if !leftErased {
+                left := "::dafny_runtime::DafnyErasable::erase_owned(" + left + ")";
+              }
+
+              if !rightErased {
+                right := "::dafny_runtime::DafnyErasable::erase_owned(" + right + ")";
+              }
+
+              match op {
+                case Eq(referential, nullable) => {
+                  if (referential) {
+                    if (nullable) {
+                      s := "::dafny_runtime::nullable_referential_equality(" + left + ", " + right + ")";
+                    } else {
+                      s := "::std::rc::Rc::ptr_eq(&(" + left + "), &(" + right + "))";
+                    }
+                  } else {
+                    s := left + " == " + right;
+                  }
+                }
+                case Neq(referential, nullable) => {
+                  if (referential) {
+                    if (nullable) {
+                      s := "!::dafny_runtime::nullable_referential_equality(" + left + ", " + right + ")";
+                    } else {
+                      s := "!::std::rc::Rc::ptr_eq(&(" + left + "), &(" + right + "))";
+                    }
+                  } else {
+                    s := left + " != " + right;
+                  }
+                }
+                case EuclidianDiv() => {
+                  s := "::dafny_runtime::euclidian_division(" + left + ", " + right + ")";
+                }
+                case Div() => {
+                  s := "(" + left + ") / (" + right + ")";
+                }
+                case EuclidianMod() => {
+                  s := "::dafny_runtime::euclidian_modulo(" + left + ", " + right + ")";
+                }
+                case Mod() => {
+                  s := "(" + left + ") % (" + right + ")";
+                }
+                case Passthrough(op) => {
+                  s := "(" + left + " " + op + " " + right + ")";
+                }
+              }
+            }
+          }
+
+          isOwned := true;
+          readIdents := recIdentsL + recIdentsR;
+          isErased := true;
+        }
         case ArrayLen(expr, dim) => {
-          var recursiveGen, _, recIdents := GenExpr(expr, selfIdent, params, OwnershipOwned);
+          var recursiveGen, _, recErased, recIdents := GenExpr(expr, selfIdent, params, true);
 
           if dim == 0 {
-            r := R.RawExpr("::dafny_runtime::BigInt::from((" + recursiveGen.ToString(IND) + ").borrow().len())");
+            s := "::dafny_runtime::BigInt::from((" + recursiveGen + ").borrow().len())";
           } else {
-            var s := R.RawExpr("::dafny_runtime::BigInt::from(m.borrow().len())").ToString(IND);
+            s := "::dafny_runtime::BigInt::from(m.borrow().len())";
             var i := 1;
             while i < dim {
               s := "m.borrow().get(0).map(|m| " + s + ").unwrap_or(::dafny_runtime::BigInt::from(0))";
               i := i + 1;
             }
 
-            r := R.RcNew(R.RawExpr("(" + recursiveGen.ToString(IND) + ")" + ".borrow().get(0).map(|m| " + s + ").unwrap_or(::dafny_runtime::BigInt::from(0))"));
+            s := "(" + recursiveGen + ")" + ".borrow().get(0).map(|m| " + s + ").unwrap_or(::dafny_runtime::BigInt::from(0))";
           }
-          r, resultingOwnership := FromOwned(r, expectedOwnership);
+
+          isOwned := true;
           readIdents := recIdents;
-          return;
-        }
-        case MapKeys(expr) => {
-          var recursiveGen, _, recIdents := GenExpr(expr, selfIdent, params, OwnershipOwned);
-          readIdents := recIdents;
-          r := R.Call(recursiveGen.Sel("keys"), [], []);
-          r, resultingOwnership := FromOwned(r, expectedOwnership);
-          return;
-        }
-        case MapValues(expr) => {
-          var recursiveGen, _, recIdents := GenExpr(expr, selfIdent, params, OwnershipOwned);
-          readIdents := recIdents;
-          r := R.Call(recursiveGen.Sel("values"), [], []);
-          r, resultingOwnership := FromOwned(r, expectedOwnership);
-          return;
+          isErased := true;
         }
         case SelectFn(on, field, isDatatype, isStatic, arity) => {
-          var onExpr, onOwned, recIdents := GenExpr(on, selfIdent, params, OwnershipBorrowed);
-          var s: string;
-          var onString := onExpr.ToString(IND);
+          var onString, onOwned, _, recIdents := GenExpr(on, selfIdent, params, false);
 
           if isStatic {
             s := onString + "::" + escapeIdent(field);
           } else {
             s := "{\n";
-            s := s + "let callTarget = (" + onString + (if onOwned == OwnershipOwned then ")" else ").clone()") + ";\n";
+            s := s + "let callTarget = (" + onString + (if onOwned then ")" else ").clone()") + ";\n";
             var args := "";
             var i := 0;
             while i < arity {
@@ -3126,144 +2319,207 @@ module {:extern "DCOMP"} DafnyToRustCompiler {
           typeShape := typeShape + ") -> _";
 
           s := "::dafny_runtime::FunctionWrapper(::std::rc::Rc::new(" + s + ") as ::std::rc::Rc<" + typeShape + ">)";
-          r := R.RawExpr(s);
-          r, resultingOwnership := FromOwned(r, expectedOwnership);
+
+          isOwned := true;
+          isErased := false;
           readIdents := recIdents;
-          return;
         }
         case Select(Companion(c), field, isConstant, isDatatype) => {
-          var onExpr, onOwned, recIdents := GenExpr(Companion(c), selfIdent, params, OwnershipBorrowed);
+          var onString, onOwned, onErased, recIdents := GenExpr(Companion(c), selfIdent, params, false);
 
-          r := R.RawExpr(onExpr.ToString(IND) + "::" + escapeIdent(field) + "()");
+          s := onString + "::" + escapeIdent(field) + "()";
 
-          r, resultingOwnership := FromOwned(r, expectedOwnership);
+          isOwned := true;
+          isErased := false;
           readIdents := recIdents;
-          return;
         }
         case Select(on, field, isConstant, isDatatype) => {
-          var onExpr, onOwned, recIdents := GenExpr(on, selfIdent, params, OwnershipBorrowed);
+          var onString, onOwned, onErased, recIdents := GenExpr(on, selfIdent, params, false);
           if isDatatype || isConstant {
-            r := R.Call(onExpr.Sel(escapeIdent(field)), [], []);
-            r, resultingOwnership := FromOwned(r, expectedOwnership);
+            s := "(" + onString + ")" + "." + escapeIdent(field) + "()";
+            if isConstant {
+              s := "&" + s;
+            }
+
+            if mustOwn {
+              s := "(" + s + ").clone()";
+              isOwned := true;
+            } else {
+              isOwned := false;
+            }
           } else {
-            var s: string;
-            s := "::std::ops::Deref::deref(&((" + onExpr.ToString(IND) + ")" + "." + escapeIdent(field) + ".borrow()))";
-            r, resultingOwnership := FromOwnership(R.RawExpr(s), OwnershipBorrowed, expectedOwnership);
+            s := "::std::ops::Deref::deref(&((" + onString + ")" + "." + escapeIdent(field) + ".borrow()))";
+            s := "(" + s + ").clone()"; // TODO(shadaj): think through when we can avoid cloning
+            isOwned := true;
           }
+
+          isErased := false;
           readIdents := recIdents;
-          return;
         }
         case Index(on, collKind, indices) => {
-          assert {:split_here} true;
-          var onExpr, onOwned, recIdents := GenExpr(on, selfIdent, params, OwnershipAutoBorrowed);
+          var onString, onOwned, onErased, recIdents := GenExpr(on, selfIdent, params, false);
           readIdents := recIdents;
-          r := onExpr;
+          // if !onErased {
+          //   var eraseFn := if onOwned then "erase_owned" else "erase";
+          //   onString := "::dafny_runtime::DafnyErasable::" + eraseFn + "(" + onString + ")";
+          // }
+
+          s := onString;
 
           var i := 0;
           while i < |indices| {
             if collKind == CollKind.Array {
-              r := r.Sel("borrow").Apply([], []);
+              s := "(" + s + ").borrow()";
             }
-            var idx, idxOwned, recIdentsIdx := GenExpr(indices[i], selfIdent, params, OwnershipBorrowed);
-            r := r.Sel("get").Apply1(idx);
-            readIdents := readIdents + recIdentsIdx;
+
+            if collKind == CollKind.Map {
+              var idx, idxOwned, idxErased, recIdentsIdx := GenExpr(indices[i], selfIdent, params, false);
+              s := "(" + s + ")[" + (if idxOwned then "&" else "") + idx + "]";
+              readIdents := readIdents + recIdentsIdx;
+            } else {
+              var idx, _, idxErased, recIdentsIdx := GenExpr(indices[i], selfIdent, params, true);
+              if !idxErased {
+                idx := "::dafny_runtime::DafnyErasable::erase_owned(" + idx + ")";
+              }
+
+              s := "(" + s + ")[<usize as ::dafny_runtime::NumCast>::from(" + idx + ").unwrap()]";
+              readIdents := readIdents + recIdentsIdx;
+            }
+
             i := i + 1;
           }
-          r, resultingOwnership := FromOwned(r, expectedOwnership);
-          return;
+
+          if mustOwn {
+            s := "(" + s + ").clone()";
+            isOwned := true;
+          } else {
+            s := "(&" + s + ")";
+            isOwned := false;
+          }
+
+          isErased := onErased;
         }
         case IndexRange(on, isArray, low, high) => {
-          var onExpr, onOwned, recIdents := GenExpr(on, selfIdent, params, OwnershipAutoBorrowed);
+          var onString, onOwned, onErased, recIdents := GenExpr(on, selfIdent, params, false);
           readIdents := recIdents;
 
-          var methodName := if low.Some? then
-            if high.Some? then "slice" else "drop"
-          else if high.Some? then "take" else "";
+          s := onString;
 
-          var arguments := [];
+          var lowString := None;
           match low {
             case Some(l) => {
-              var lExpr, _, recIdentsL := GenExpr(l, selfIdent, params, OwnershipBorrowed);
-              arguments := arguments + [lExpr];
+              var lString, _, lErased, recIdentsL := GenExpr(l, selfIdent, params, true);
+              if !lErased {
+                lString := "::dafny_runtime::DafnyErasable::erase_owned(" + lString + ")";
+              }
+
+              lowString := Some(lString);
               readIdents := readIdents + recIdentsL;
             }
             case None => {}
           }
 
+          var highString := None;
           match high {
             case Some(h) => {
-              var hExpr, _, recIdentsH := GenExpr(h, selfIdent, params, OwnershipBorrowed);
-              arguments := arguments + [hExpr];
+              var hString, _, hErased, recIdentsH := GenExpr(h, selfIdent, params, true);
+              if !hErased {
+                hString := "::dafny_runtime::DafnyErasable::erase_owned(" + hString + ")";
+              }
+
+              highString := Some(hString);
               readIdents := readIdents + recIdentsH;
             }
             case None => {}
           }
 
-          r := onExpr;
           if isArray {
-            if methodName != "" {
-              methodName := "_" + methodName;
-            }
-            r := R.dafny_runtime_Sequence.MSel("from_array"+methodName).Apply([], arguments);
-          } else {
-            if methodName != "" {
-              r := r.Sel(methodName).Apply([], arguments);
-            }
+            s := "(" + s + ").borrow()";
           }
-          r, resultingOwnership := FromOwned(r, expectedOwnership);
-          return;
+
+          s := "(" + s + ")" + "[" + (match lowString {
+                                        case Some(l) => "<usize as ::dafny_runtime::NumCast>::from(" + l + ").unwrap()"
+                                        case None => ""
+                                      }) + ".." + (match highString {
+                                                     case Some(h) => "<usize as ::dafny_runtime::NumCast>::from(" + h + ").unwrap()"
+                                                     case None => ""
+                                                   }) + "]";
+
+          isErased := onErased;
+
+          s := "(" + s + ".to_vec())";
+          isOwned := true;
         }
         case TupleSelect(on, idx) => {
-          var onExpr, onOwnership, recIdents := GenExpr(on, selfIdent, params, OwnershipAutoBorrowed);
-          r := onExpr.Sel(Strings.OfNat(idx));
-          r, resultingOwnership := FromOwnership(r, onOwnership, expectedOwnership);
+          var onString, _, tupErased, recIdents := GenExpr(on, selfIdent, params, false);
+          s := "(" + onString + ")." + Strings.OfNat(idx);
+          if mustOwn {
+            s := "(" + s + ")" + ".clone()";
+            isOwned := true;
+          } else {
+            s := "&" + s;
+            isOwned := false;
+          }
+          isErased := tupErased;
           readIdents := recIdents;
-          return;
         }
         case Call(on, name, typeArgs, args) => {
           readIdents := {};
 
-          var typeExprs := [];
+          var typeArgString := "";
           if (|typeArgs| >= 1) {
             var typeI := 0;
+            typeArgString := "::<";
             while typeI < |typeArgs| {
+              if typeI > 0 {
+                typeArgString := typeArgString + ", ";
+              }
 
-              var typeExpr := GenType(typeArgs[typeI], false, false);
-              typeExprs := typeExprs + [typeExpr];
+              var typeString := GenType(typeArgs[typeI], false, false);
+              typeArgString := typeArgString + typeString;
 
               typeI := typeI + 1;
             }
+            typeArgString := typeArgString + ">";
           }
 
-          var argExprs := [];
+          var argString := "";
           var i := 0;
           while i < |args| {
-            var argExpr, argOwnership, argIdents := GenExpr(args[i], selfIdent, params, OwnershipBorrowed);
-            argExprs := argExprs + [argExpr];
+            if i > 0 {
+              argString := argString + ", ";
+            }
+
+            var argExpr, isOwned, argErased, argIdents := GenExpr(args[i], selfIdent, params, false);
+            if isOwned {
+              argExpr := "&(" + argExpr + ")";
+            }
+
+            if !argErased {
+              argExpr := "::dafny_runtime::DafnyErasable::erase(" + argExpr + ")";
+            }
+            argExpr := "::dafny_runtime::DafnyUnerasable::unerase(" + argExpr + ")";
+
+            argString := argString + argExpr;
             readIdents := readIdents + argIdents;
 
             i := i + 1;
           }
 
-          var onExpr, _, recIdents := GenExpr(on, selfIdent, params, OwnershipAutoBorrowed);
+          var enclosingString, _, _, recIdents := GenExpr(on, selfIdent, params, false);
           readIdents := readIdents + recIdents;
-          var renderedName := match name {
-            case Name(ident) => escapeIdent(ident)
-            case MapBuilderAdd | SetBuilderAdd => "add"
-            case MapBuilderBuild | SetBuilderBuild => "build"
-          };
           match on {
             case Companion(_) => {
-              onExpr := onExpr.MSel(renderedName);
+              enclosingString := enclosingString + "::" + escapeIdent(name.id);
             }
             case _ => {
-              onExpr := onExpr.Sel(renderedName);
+              enclosingString := "(" + enclosingString + ")." + escapeIdent(name.id);
             }
           }
 
-          r := R.Call(onExpr, typeExprs, argExprs);
-          r, resultingOwnership := FromOwned(r, expectedOwnership);
-          return;
+          s := enclosingString + typeArgString + "(" + argString + ")";
+          isOwned := true;
+          isErased := false;
         }
         case Lambda(params, retType, body) => {
           var paramNames := [];
@@ -3273,7 +2529,7 @@ module {:extern "DCOMP"} DafnyToRustCompiler {
             i := i + 1;
           }
 
-          var recursiveGen, recIdents := GenStmts(body, if selfIdent != None then Some("_this") else None, paramNames, true, R.RawExpr(""));
+          var recursiveGen, recIdents := GenStmts(body, if selfIdent != None then Some("_this") else None, paramNames, true, "");
           readIdents := {};
           var allReadCloned := "";
           while recIdents != {} decreases recIdents {
@@ -3302,16 +2558,16 @@ module {:extern "DCOMP"} DafnyToRustCompiler {
 
             var typStr := GenType(params[i].typ, false, true);
 
-            paramsString := paramsString + escapeIdent(params[i].name) + ": " + R.Borrowed(typStr).ToString(IND);
-            paramTypes := paramTypes + R.Borrowed(typStr).ToString(IND);
+            paramsString := paramsString + escapeIdent(params[i].name) + ": &" + typStr;
+            paramTypes := paramTypes + "&" + typStr;
             i := i + 1;
           }
 
           var retTypeGen := GenType(retType, false, true);
 
-          r := R.RawExpr("::dafny_runtime::FunctionWrapper::<::std::rc::Rc<dyn ::std::ops::Fn(" + paramTypes + ") -> " + retTypeGen.ToString(IND) + ">>({\n" + allReadCloned + "::std::rc::Rc::new(move |" + paramsString + "| -> " + retTypeGen.ToString(IND) + " {\n" + recursiveGen.ToString(IND) + "\n})})");
-          r, resultingOwnership := FromOwned(r, expectedOwnership);
-          return;
+          s := "::dafny_runtime::FunctionWrapper::<::std::rc::Rc<dyn ::std::ops::Fn(" + paramTypes + ") -> " + retTypeGen + ">>({\n" + allReadCloned + "::std::rc::Rc::new(move |" + paramsString + "| -> " + retTypeGen + " {\n" + recursiveGen + "\n})})";
+          isOwned := true;
+          isErased := false;
         }
         case BetaRedex(values, retType, expr) => {
           var paramNames := [];
@@ -3324,7 +2580,7 @@ module {:extern "DCOMP"} DafnyToRustCompiler {
           }
 
           readIdents := {};
-          var s := "{\n";
+          s := "{\n";
 
           var paramsString := "";
           i := 0;
@@ -3335,36 +2591,41 @@ module {:extern "DCOMP"} DafnyToRustCompiler {
 
             var typStr := GenType(values[i].0.typ, false, true);
 
-            var valueGen, _, recIdents := GenExpr(values[i].1, selfIdent, params, OwnershipOwned);
-            s := s + "let " + escapeIdent(values[i].0.name) + ": " + typStr.ToString(IND) + " = ";
+            var valueGen, _, valueErased, recIdents := GenExpr(values[i].1, selfIdent, params, true);
+            s := s + "let " + escapeIdent(values[i].0.name) + ": " + typStr + " = ";
             readIdents := readIdents + recIdents;
+            if valueErased {
+              valueGen := "::dafny_runtime::DafnyUnerasable::<_>::unerase_owned" + "(" + valueGen + ")";
+            }
 
-            s := s + valueGen.ToString(IND) + ";\n";
+            s := s + valueGen + ";\n";
             i := i + 1;
           }
 
-          var recGen, recOwned, recIdents := GenExpr(expr, selfIdent, paramNames, expectedOwnership);
+          var recGen, recOwned, recErased, recIdents := GenExpr(expr, selfIdent, paramNames, mustOwn);
           readIdents := recIdents - paramNamesSet;
 
-          s := s  + recGen.ToString(IND) + "\n}";
-          r := R.RawExpr(s);
-          r, resultingOwnership := FromOwnership(r, recOwned, expectedOwnership);
-          return;
+          s := s  + recGen + "\n}";
+          isOwned := recOwned;
+          isErased := recErased;
         }
         case IIFE(name, tpe, value, iifeBody) => {
-          var valueGen, _, recIdents := GenExpr(value, selfIdent, params, OwnershipOwned);
+          var valueGen, _, valueErased, recIdents := GenExpr(value, selfIdent, params, true);
+          if valueErased {
+            valueGen := "::dafny_runtime::DafnyUnerasable::<_>::unerase_owned" + "(" + valueGen + ")";
+          }
 
           readIdents := recIdents;
           var valueTypeGen := GenType(tpe, false, true);
-          var bodyGen, _, bodyIdents := GenExpr(iifeBody, selfIdent, params, OwnershipOwned);
+          var bodyGen, _, bodyErased, bodyIdents := GenExpr(iifeBody, selfIdent, params, true);
           readIdents := readIdents + (bodyIdents - {name.id});
 
-          r := R.RawExpr("{\nlet " + escapeIdent(name.id) + ": " + valueTypeGen.ToString(IND) + " = " + valueGen.ToString(IND) + ";\n" + bodyGen.ToString(IND) + "\n}");
-          r, resultingOwnership := FromOwned(r, expectedOwnership);
-          return;
+          s := "{\nlet " + escapeIdent(name.id) + ": " + valueTypeGen + " = " + valueGen + ";\n" + bodyGen + "\n}";
+          isOwned := true;
+          isErased := bodyErased;
         }
         case Apply(func, args) => {
-          var funcExpr, _, recIdents := GenExpr(func, selfIdent, params, OwnershipBorrowed);
+          var funcString, _, funcErased, recIdents := GenExpr(func, selfIdent, params, false);
           readIdents := recIdents;
 
           var argString := "";
@@ -3374,82 +2635,73 @@ module {:extern "DCOMP"} DafnyToRustCompiler {
               argString := argString + ", ";
             }
 
-            var argExpr, argOwned, argIdents := GenExpr(args[i], selfIdent, params, OwnershipBorrowed);
-            var argExprString := argExpr.ToString(IND);
-            if argOwned == OwnershipOwned {
-              argExprString := "&" + argExprString;
+            var argExpr, isOwned, argErased, argIdents := GenExpr(args[i], selfIdent, params, false);
+            if isOwned {
+              argExpr := "&" + argExpr;
             }
 
-            argString := argString + argExprString;
+            argString := argString + argExpr;
             readIdents := readIdents + argIdents;
 
             i := i + 1;
           }
 
-          r := R.RawExpr("((" + funcExpr.ToString(IND) + ").0" + "(" + argString + "))");
-          r, resultingOwnership := FromOwned(r, expectedOwnership);
-          return;
+          s := "((" + funcString + ").0" + "(" + argString + "))";
+          isOwned := true;
+          isErased := false;
         }
         case TypeTest(on, dType, variant) => {
-          var exprGen, _, recIdents := GenExpr(on, selfIdent, params, OwnershipBorrowed);
+          var exprGen, _, exprErased, recIdents := GenExpr(on, selfIdent, params, false);
           var dTypePath := GenPath(dType);
-          r := R.RawExpr("matches!(" + exprGen.ToString(IND) + ".as_ref(), " + dTypePath + "::" + escapeIdent(variant) + "{ .. })");
-          r, resultingOwnership := FromOwned(r, expectedOwnership);
+          s := "matches!(" + exprGen + ".as_ref(), " + dTypePath + "::" + escapeIdent(variant) + "{ .. })";
+          isOwned := true;
+          isErased := true;
           readIdents := recIdents;
-          return;
         }
         case BoolBoundedPool() => {
-          r := R.RawExpr("[false, true]");
-          r, resultingOwnership := FromOwned(r, expectedOwnership);
+          s := "[false, true]";
+          isOwned := true;
+          isErased := true;
           readIdents := {};
-          return;
         }
         case SetBoundedPool(of) => {
-          var exprGen, _, recIdents := GenExpr(of, selfIdent, params, OwnershipBorrowed);
-          r := R.RawExpr("(" + exprGen.ToString(IND) + ").iter()");
-          r, resultingOwnership := FromOwned(r, expectedOwnership);
+          var exprGen, _, exprErased, recIdents := GenExpr(of, selfIdent, params, false);
+          s := "(" + exprGen + ").iter()";
+          isOwned := true;
+          isErased := exprErased;
           readIdents := recIdents;
-          return;
         }
         case SeqBoundedPool(of, includeDuplicates) => {
-          var exprGen, _, recIdents := GenExpr(of, selfIdent, params, OwnershipBorrowed);
-          var s := "(" + exprGen.ToString(IND) + ").iter()";
+          var exprGen, _, exprErased, recIdents := GenExpr(of, selfIdent, params, false);
+          s := "(" + exprGen + ").iter()";
           if !includeDuplicates {
             s := "::dafny_runtime::itertools::Itertools::unique(" + s + ")";
           }
-          r := R.RawExpr(s);
-          r, resultingOwnership := FromOwned(r, expectedOwnership);
+          isOwned := true;
+          isErased := exprErased;
           readIdents := recIdents;
-          return;
         }
         case IntRange(lo, hi) => {
-          var lo, _, recIdentsLo := GenExpr(lo, selfIdent, params, OwnershipOwned);
-          var hi, _, recIdentsHi := GenExpr(hi, selfIdent, params, OwnershipOwned);
+          var loString, _, loErased, recIdentsLo := GenExpr(lo, selfIdent, params, true);
+          var hiString, _, hiErased, recIdentsHi := GenExpr(hi, selfIdent, params, true);
 
-          r := R.RawExpr("::dafny_runtime::integer_range(" + lo.ToString(IND) + ", " + hi.ToString(IND) + ")");
-          r, resultingOwnership := FromOwned(r, expectedOwnership);
+          if !loErased {
+            loString := "::dafny_runtime::DafnyErasable::erase_owned(" + loString + ")";
+          }
+
+          if !hiErased {
+            hiString := "::dafny_runtime::DafnyErasable::erase_owned(" + hiString + ")";
+          }
+
+          s := "::dafny_runtime::integer_range(" + loString + ", " + hiString + ")";
+          isOwned := true;
+          isErased := true;
           readIdents := recIdentsLo + recIdentsHi;
-          return;
-        }
-        case MapBuilder(keyType, valueType) => {
-          var kType := GenType(keyType, false, false);
-          var vType := GenType(valueType, false, false);
-          r := R.RawExpr("::dafny_runtime::MapBuilder::<" + kType.ToString(IND) + ", " + vType.ToString(IND) + ">::new()");
-          r, resultingOwnership := FromOwned(r, expectedOwnership);
-          readIdents := {};
-          return;
-        }
-        case SetBuilder(elemType) => {
-          var eType := GenType(elemType, false, false);
-          readIdents := {};
-          r := R.RawExpr("::dafny_runtime::SetBuilder::<" + eType.ToString(IND) + ">::new()");
-          r, resultingOwnership := FromOwned(r, expectedOwnership);
-          return;
         }
       }
     }
 
-    method Compile(p: seq<Module>) returns (s: string) {
+    static method Compile(p: seq<Module>) returns (s: string) {
       s := "#![allow(warnings, unconditional_panic)]\n";
       s := s + "#![allow(nonstandard_style)]\n";
       s := s + "extern crate dafny_runtime;\n";
